examples/Derived_Patterns.thy
@@ -1,51 +1,136 @@
 theory Derived_Patterns imports Patterns
-begin
-
+ begin
 definition always2 where "always2 A11 A12 A2 s \<equiv> (always (\<lambda> r2 r1 . ((weak_previous (\<lambda> r4 r3 . (\<not> (A11 r3))) r2 r1) \<or> ((\<not> (A12 r1)) \<or> (A2 r2 r1)))) s)"
 
 definition always2_part where "always2_part A11 A12 A2 s \<equiv> (always2 A11 A12 (\<lambda> s s1 . (A2 s1)) s)"
 
-definition always2_inv where "always2_inv b_0 A11 A12 A2_1 s \<equiv> ((always_inv (\<lambda> r2 r1 . ((weak_previous (\<lambda> r4 r3 . (\<not> (A11 r3))) r2 r1) \<or> ((\<not> (A12 r1)) \<or> (A2_1 r2 r1)))) s) \<and> (b_0 s --> (previous_inv (\<lambda> r4 r3 . (\<not> (A11 r3))) s)))"
+definition always2_inv where "always2_inv b_0 A11 A12 A2_1 s \<equiv> ((always_inv (\<lambda> r2 r1 . ((weak_previous (\<lambda> r4 r3 . (\<not> (A11 r3))) r2 r1) \<or> ((\<not> (A12 r1)) \<or> (A2_1 r2 r1)))) s) \<and> (previous_inv b_0 (\<lambda> r4 r3 . (\<not> (A11 r3))) s))"
 
 definition always2_inv_part where "always2_inv_part b_0 A11 A12 A2 s \<equiv> (always2_inv b_0 A11 A12 (\<lambda> s s1 . (A2 s1)) s)"
-
-
 
 lemma always2_inv_saving_gen: "
 always2_inv b_0 A11 A12 A2_1 s0 \<Longrightarrow>
 consecutive s0 s \<Longrightarrow>
 (((True \<and> (True \<and> (always_imp s0 (\<lambda> r1 . (A2_1 s0 r1)) (\<lambda> r1 . (A2_1 s r1))))) \<and> (((b_0 s0) \<and> True) \<or> ((\<not> (A12 s)) \<or> (A2_1 s s)))) \<and> ((b_0 s) --> (\<not> (A11 s)))) \<Longrightarrow>
 always2_inv b_0 A11 A12 A2_1 s"
-  unfolding always2_inv_def
-  apply(proveOuter add_rules: invsaving)
+unfolding always2_inv_def
+apply(erule conjE)
+apply(erule conjE)
+subgoal premises prems1
+apply(rule conjI)
+apply(insert prems1(1,2,4))[1]
+apply(erule always_rule)
+  apply simp
+  apply(erule conjE)
+  subgoal premises prems2
+  apply(rule conjI)
+  apply(insert prems2(1,2))[1]
+    apply(rule always_disj_rule)
+    apply simp
+      apply(erule conjE)
+      subgoal premises prems3
+      apply(rule conjI)
+      apply(insert prems3(1,2))[1]
+        apply(rule weak_previous_LS4)
+        apply simp
+          apply(rule always_imp_refl)
+      apply(insert prems3(1,3))
+        apply(rule always_disj_rule)
+        apply simp
+          apply(erule conjE)
+          subgoal premises prems4
+          apply(rule conjI)
+          apply(insert prems4(1,2))[1]
+            apply(rule always_imp_refl)
+          apply(insert prems4(1,3))
+            apply assumption
+          done
+      done
+  apply(insert prems2(1,3))
+    apply(erule disjE)
+    apply(rule disjI1)
+      apply(rule weak_previous_one_point[OF prems1(3)])
+      apply simp
+        apply(erule conjE)
+        subgoal premises prems5
+        apply(rule conjI)
+        apply(insert prems5(1,2))[1]
+          apply assumption
+        apply(insert prems5(1,3))
+          apply(rule always_imp_refl)
+        done
+    apply(rule disjI2)
+      apply(erule disjE)
+      apply(rule disjI1)
+        apply assumption
+      apply(rule disjI2)
+        apply assumption
   done
+apply(insert prems1(1,3,5))
+  apply(erule previous_rule)
+  apply simp
+  apply(rule impI)
+  apply(erule impE)
+  apply assumption
+  subgoal premises prems6
+  apply(insert prems6(1,3))
+    apply assumption
+  done
+done
+done
 
 lemma always2einv_imp_req_gen: "
 always2_inv b_0 A11 A12 A2_1 s0 \<Longrightarrow>
 toEnvP s0 \<Longrightarrow>
 (True \<and> (True \<and> (always_imp s0 (\<lambda> r1 . (A2_1 s0 r1)) (\<lambda> r1 . (A2 s0 r1))))) \<Longrightarrow>
-always2 A11 A12 A2 s0"
-  unfolding always2_inv_def always2_def
-  apply(proveOuter add_rules: inv_req)
-  done
+always2 A11 A12 A2 s0"unfolding always2_inv_def always2_def
+subgoal premises prems1
+apply(insert prems1(1,2))
+apply(erule conjE)
+subgoal premises prems2
+apply(insert prems2(1,2) prems1(3))
+apply(erule always_einv2req)
+apply simp
+  apply(rule always_disj_rule)
+  apply simp
+    apply(erule conjE)
+    subgoal premises prems3
+    apply(rule conjI)
+    apply(insert prems3(1,2))[1]
+      apply(rule weak_previous_LS5)
+      apply simp
+        apply(rule always_imp_refl)
+    apply(insert prems3(1,3))
+      apply(rule always_disj_rule)
+      apply simp
+        apply(erule conjE)
+        subgoal premises prems4
+        apply(rule conjI)
+        apply(insert prems4(1,2))[1]
+          apply(rule always_imp_refl)
+        apply(insert prems4(1,3))
+          apply assumption
+        done
+    done
+done
+done
+done
 
 lemma always2_inv_saving: "
 always2_inv_part b_0 A11 A12 A2 s0 \<Longrightarrow>
 consecutive s0 s \<Longrightarrow>
 (((b_0 s0) \<or> ((\<not> (A12 s)) \<or> (A2 s))) \<and> ((b_0 s) --> (\<not> (A11 s)))) \<Longrightarrow>
-always2_inv_part b_0 A11 A12 A2 s"
-  unfolding always2_inv_part_def
-  apply(auto simp add: always2_inv_saving_gen always_imp_refl)
-  done
+always2_inv_part b_0 A11 A12 A2 s"unfolding always2_inv_part_def always2_part_def
+apply(simp add: always2_inv_saving_gen always_imp_refl)
+done
 
 lemma always2einv_imp_req: "
 always2_inv_part b_0 A11 A12 A2 s \<Longrightarrow>
 toEnvP s \<Longrightarrow>
 True \<Longrightarrow>
-always2_part A11 A12 A2 s"
-  unfolding always2_inv_part_def always2_part_def
-  apply(auto simp add: always2einv_imp_req_gen always_imp_refl)
-  done
+always2_part A11 A12 A2 s"unfolding always2_inv_part_def always2_part_def
+apply(simp add: always2einv_imp_req_gen always_imp_refl)
+done
 
 lemmas always2_used_patterns = always2_def always_def weak_previous_def 
 
@@ -55,8 +140,6 @@ lemmas always2_inv_part_used_patterns = always2_inv_part_def always2_inv_used_pa
 
 lemmas always2_part_used_patterns = always2_part_def always2_used_patterns
 
-
-
 definition P1_1 where "P1_1 t A1 A2 A3 s \<equiv> (always (\<lambda> r2 r1 . ((\<not> (A1 r1)) \<or> (constrained_until t A2 A3 r2 r1))) s)"
 
 definition P1_1_part where "P1_1_part t A1 A2 A3 s \<equiv> (P1_1 t A1 (\<lambda> s s1 . (A2 s1)) (\<lambda> s s1 . (A3 s1)) s)"
@@ -65,43 +148,138 @@ definition P1_1_inv where "P1_1_inv t t1_0 A1 A2_1 A3_1 s \<equiv> (always_inv (
 
 definition P1_1_inv_part where "P1_1_inv_part t t1_0 A1 A2 A3 s \<equiv> (P1_1_inv t t1_0 A1 (\<lambda> s s1 . (A2 s1)) (\<lambda> s s1 . (A3 s1)) s)"
 
-
-
 lemma P1_1_inv_saving_gen: "
 P1_1_inv t t1_0 A1 A2_1 A3_1 s0 \<Longrightarrow>
 consecutive s0 s \<Longrightarrow>
 ((True \<and> ((always_imp s0 (A2_1 s0) (A2_1 s)) \<and> ((always_imp s0 (A3_1 s0) (A3_1 s)) \<and> (((t1_0 s0) = 0) \<or> (((A3_1 s s) \<and> ((t1_0 s0) <= t)) \<or> ((A2_1 s s) \<and> ((t1_0 s0) < (t1_0 s)))))))) \<and> ((\<not> (A1 s)) \<or> ((A3_1 s s) \<or> ((A2_1 s s) \<and> ((t1_0 s) > 0))))) \<Longrightarrow>
 P1_1_inv t t1_0 A1 A2_1 A3_1 s"
-  unfolding P1_1_inv_def
-  apply(proveOuter add_rules: invsaving)
+unfolding P1_1_inv_def
+apply(erule always_rule)
+  apply simp
+  apply(erule conjE)
+  subgoal premises prems1
+  apply(rule conjI)
+  apply(insert prems1(1,2))[1]
+    apply(rule always_disj_rule)
+    apply simp
+      apply(erule conjE)
+      subgoal premises prems2
+      apply(rule conjI)
+      apply(insert prems2(1,2))[1]
+        apply(rule always_imp_refl)
+      apply(insert prems2(1,3))
+        apply(rule constrained_until_rule)
+        apply simp
+          apply(erule conjE)
+          subgoal premises prems3
+          apply(rule conjI)
+          apply(insert prems3(1,2))[1]
+            apply assumption
+          apply(insert prems3(1,3))
+            apply(erule conjE)
+            subgoal premises prems4
+            apply(rule conjI)
+            apply(insert prems4(1,2))[1]
+              apply assumption
+            apply(insert prems4(1,3))
+              apply(erule disjE)
+              apply(rule disjI1)
+                apply assumption
+              apply(rule disjI2)
+                apply(erule disjE)
+                apply(rule disjI1)
+                  apply(erule conjE)
+                  subgoal premises prems5
+                  apply(rule conjI)
+                  apply(insert prems5(1,2))[1]
+                    apply assumption
+                  apply(insert prems5(1,3))
+                    apply assumption
+                  done
+                apply(rule disjI2)
+                  apply(erule conjE)
+                  subgoal premises prems6
+                  apply(rule conjI)
+                  apply(insert prems6(1,2))[1]
+                    apply assumption
+                  apply(insert prems6(1,3))
+                    apply assumption
+                  done
+            done
+          done
+      done
+  apply(insert prems1(1,3))
+    apply(erule disjE)
+    apply(rule disjI1)
+      apply assumption
+    apply(rule disjI2)
+      apply(rule constrained_until_one_point)
+      apply simp
+        apply(erule disjE)
+        apply(rule disjI1)
+          apply assumption
+        apply(rule disjI2)
+          apply(erule conjE)
+          subgoal premises prems7
+          apply(rule conjI)
+          apply(insert prems7(1,2))[1]
+            apply assumption
+          apply(insert prems7(1,3))
+            apply assumption
+          done
   done
+done
 
 lemma P1_1einv_imp_req_gen: "
 P1_1_inv t t1_0 A1 A2_1 A3_1 s0 \<Longrightarrow>
 toEnvP s0 \<Longrightarrow>
 (True \<and> ((always_imp s0 (A2_1 s0) (A2 s0)) \<and> ((always_imp s0 (A3_1 s0) (A3 s0)) \<and> ((t1_0 s0) <= t)))) \<Longrightarrow>
-P1_1 t A1 A2 A3 s0"
-  unfolding P1_1_inv_def P1_1_def
-  apply(proveOuter add_rules:inv_req)
-  done
+P1_1 t A1 A2 A3 s0"unfolding P1_1_inv_def P1_1_def
+apply(erule always_einv2req)
+apply simp
+  apply(rule always_disj_rule)
+  apply simp
+    apply(erule conjE)
+    subgoal premises prems3
+    apply(rule conjI)
+    apply(insert prems3(1,2))[1]
+      apply(rule always_imp_refl)
+    apply(insert prems3(1,3))
+      apply(rule constrained_until_einv2req)
+      apply simp
+        apply(erule conjE)
+        subgoal premises prems4
+        apply(rule conjI)
+        apply(insert prems4(1,2))[1]
+          apply assumption
+        apply(insert prems4(1,3))
+          apply(erule conjE)
+          subgoal premises prems5
+          apply(rule conjI)
+          apply(insert prems5(1,2))[1]
+            apply assumption
+          apply(insert prems5(1,3))
+            apply assumption
+          done
+        done
+    done
+done
 
 lemma P1_1_inv_saving: "
 P1_1_inv_part t t1_0 A1 A2 A3 s0 \<Longrightarrow>
 consecutive s0 s \<Longrightarrow>
 ((((t1_0 s0) = 0) \<or> (((A3 s) \<and> ((t1_0 s0) <= t)) \<or> ((A2 s) \<and> ((t1_0 s0) < (t1_0 s))))) \<and> ((\<not> (A1 s)) \<or> ((A3 s) \<or> ((A2 s) \<and> ((t1_0 s) > 0))))) \<Longrightarrow>
-P1_1_inv_part t t1_0 A1 A2 A3 s"
-  unfolding P1_1_inv_part_def
-  apply(simp add: P1_1_inv_saving_gen always_imp_refl)
-  done
+P1_1_inv_part t t1_0 A1 A2 A3 s"unfolding P1_1_inv_part_def P1_1_part_def
+apply(simp add: P1_1_inv_saving_gen always_imp_refl)
+done
 
 lemma P1_1einv_imp_req: "
 P1_1_inv_part t t1_0 A1 A2 A3 s \<Longrightarrow>
 toEnvP s \<Longrightarrow>
 ((t1_0 s) <= t) \<Longrightarrow>
-P1_1_part t A1 A2 A3 s"
-  unfolding P1_1_inv_part_def P1_1_part_def
-  apply(auto simp add: P1_1einv_imp_req_gen always_imp_refl)
-  done
+P1_1_part t A1 A2 A3 s"unfolding P1_1_inv_part_def P1_1_part_def
+apply(simp add: P1_1einv_imp_req_gen always_imp_refl)
+done
 
 lemmas P1_1_used_patterns = P1_1_def always_def constrained_until_def 
 
@@ -111,53 +289,204 @@ lemmas P1_1_inv_part_used_patterns = P1_1_inv_part_def P1_1_inv_used_patterns
 
 lemmas P1_1_part_used_patterns = P1_1_part_def P1_1_used_patterns
 
-
-
 definition P1_2 where "P1_2 t A11 A12 A2 A3 s \<equiv> (always (\<lambda> r2 r1 . ((weak_previous (\<lambda> r4 r3 . (\<not> (A11 r3))) r2 r1) \<or> ((\<not> (A12 r1)) \<or> (constrained_until t A2 A3 r2 r1)))) s)"
 
 definition P1_2_part where "P1_2_part t A11 A12 A2 A3 s \<equiv> (P1_2 t A11 A12 (\<lambda> s s1 . (A2 s1)) (\<lambda> s s1 . (A3 s1)) s)"
 
-definition P1_2_inv where "P1_2_inv t b_0 t1_0 A11 A12 A2_1 A3_1 s \<equiv> ((always_inv (\<lambda> r2 r1 . ((weak_previous (\<lambda> r4 r3 . (\<not> (A11 r3))) r2 r1) \<or> ((\<not> (A12 r1)) \<or> (constrained_until_inv t t1_0 A2_1 A3_1 r2 r1)))) s) \<and> (b_0 s --> (previous_inv (\<lambda> r4 r3 . (\<not> (A11 r3))) s)))"
+definition P1_2_inv where "P1_2_inv t b_0 t1_0 A11 A12 A2_1 A3_1 s \<equiv> ((always_inv (\<lambda> r2 r1 . ((weak_previous (\<lambda> r4 r3 . (\<not> (A11 r3))) r2 r1) \<or> ((\<not> (A12 r1)) \<or> (constrained_until_inv t t1_0 A2_1 A3_1 r2 r1)))) s) \<and> (previous_inv b_0 (\<lambda> r4 r3 . (\<not> (A11 r3))) s))"
 
 definition P1_2_inv_part where "P1_2_inv_part t b_0 t1_0 A11 A12 A2 A3 s \<equiv> (P1_2_inv t b_0 t1_0 A11 A12 (\<lambda> s s1 . (A2 s1)) (\<lambda> s s1 . (A3 s1)) s)"
-
-
 
 lemma P1_2_inv_saving_gen: "
 P1_2_inv t b_0 t1_0 A11 A12 A2_1 A3_1 s0 \<Longrightarrow>
 consecutive s0 s \<Longrightarrow>
 (((True \<and> (True \<and> ((always_imp s0 (A2_1 s0) (A2_1 s)) \<and> ((always_imp s0 (A3_1 s0) (A3_1 s)) \<and> (((t1_0 s0) = 0) \<or> (((A3_1 s s) \<and> ((t1_0 s0) <= t)) \<or> ((A2_1 s s) \<and> ((t1_0 s0) < (t1_0 s))))))))) \<and> (((b_0 s0) \<and> True) \<or> ((\<not> (A12 s)) \<or> ((A3_1 s s) \<or> ((A2_1 s s) \<and> ((t1_0 s) > 0)))))) \<and> ((b_0 s) --> (\<not> (A11 s)))) \<Longrightarrow>
 P1_2_inv t b_0 t1_0 A11 A12 A2_1 A3_1 s"
-  unfolding P1_2_inv_def
-  apply(proveOuter add_rules: invsaving)
+unfolding P1_2_inv_def
+apply(erule conjE)
+apply(erule conjE)
+subgoal premises prems1
+apply(rule conjI)
+apply(insert prems1(1,2,4))[1]
+apply(erule always_rule)
+  apply simp
+  apply(erule conjE)
+  subgoal premises prems2
+  apply(rule conjI)
+  apply(insert prems2(1,2))[1]
+    apply(rule always_disj_rule)
+    apply simp
+      apply(erule conjE)
+      subgoal premises prems3
+      apply(rule conjI)
+      apply(insert prems3(1,2))[1]
+        apply(rule weak_previous_LS4)
+        apply simp
+          apply(rule always_imp_refl)
+      apply(insert prems3(1,3))
+        apply(rule always_disj_rule)
+        apply simp
+          apply(erule conjE)
+          subgoal premises prems4
+          apply(rule conjI)
+          apply(insert prems4(1,2))[1]
+            apply(rule always_imp_refl)
+          apply(insert prems4(1,3))
+            apply(rule constrained_until_rule)
+            apply simp
+              apply(erule conjE)
+              subgoal premises prems5
+              apply(rule conjI)
+              apply(insert prems5(1,2))[1]
+                apply assumption
+              apply(insert prems5(1,3))
+                apply(erule conjE)
+                subgoal premises prems6
+                apply(rule conjI)
+                apply(insert prems6(1,2))[1]
+                  apply assumption
+                apply(insert prems6(1,3))
+                  apply(erule disjE)
+                  apply(rule disjI1)
+                    apply assumption
+                  apply(rule disjI2)
+                    apply(erule disjE)
+                    apply(rule disjI1)
+                      apply(erule conjE)
+                      subgoal premises prems7
+                      apply(rule conjI)
+                      apply(insert prems7(1,2))[1]
+                        apply assumption
+                      apply(insert prems7(1,3))
+                        apply assumption
+                      done
+                    apply(rule disjI2)
+                      apply(erule conjE)
+                      subgoal premises prems8
+                      apply(rule conjI)
+                      apply(insert prems8(1,2))[1]
+                        apply assumption
+                      apply(insert prems8(1,3))
+                        apply assumption
+                      done
+                done
+              done
+          done
+      done
+  apply(insert prems2(1,3))
+    apply(erule disjE)
+    apply(rule disjI1)
+      apply(rule weak_previous_one_point[OF prems1(3)])
+      apply simp
+        apply(erule conjE)
+        subgoal premises prems9
+        apply(rule conjI)
+        apply(insert prems9(1,2))[1]
+          apply assumption
+        apply(insert prems9(1,3))
+          apply(rule always_imp_refl)
+        done
+    apply(rule disjI2)
+      apply(erule disjE)
+      apply(rule disjI1)
+        apply assumption
+      apply(rule disjI2)
+        apply(rule constrained_until_one_point)
+        apply simp
+          apply(erule disjE)
+          apply(rule disjI1)
+            apply assumption
+          apply(rule disjI2)
+            apply(erule conjE)
+            subgoal premises prems10
+            apply(rule conjI)
+            apply(insert prems10(1,2))[1]
+              apply assumption
+            apply(insert prems10(1,3))
+              apply assumption
+            done
   done
+apply(insert prems1(1,3,5))
+  apply(erule previous_rule)
+  apply simp
+  apply(rule impI)
+  apply(erule impE)
+  apply assumption
+  subgoal premises prems11
+  apply(insert prems11(1,3))
+    apply assumption
+  done
+done
+done
 
 lemma P1_2einv_imp_req_gen: "
 P1_2_inv t b_0 t1_0 A11 A12 A2_1 A3_1 s0 \<Longrightarrow>
 toEnvP s0 \<Longrightarrow>
 (True \<and> (True \<and> ((always_imp s0 (A2_1 s0) (A2 s0)) \<and> ((always_imp s0 (A3_1 s0) (A3 s0)) \<and> ((t1_0 s0) <= t))))) \<Longrightarrow>
-P1_2 t A11 A12 A2 A3 s0"
-  unfolding P1_2_inv_def P1_2_def
-  apply(proveOuter add_rules: inv_req)
-  done
+P1_2 t A11 A12 A2 A3 s0"unfolding P1_2_inv_def P1_2_def
+subgoal premises prems1
+apply(insert prems1(1,2))
+apply(erule conjE)
+subgoal premises prems2
+apply(insert prems2(1,2) prems1(3))
+apply(erule always_einv2req)
+apply simp
+  apply(rule always_disj_rule)
+  apply simp
+    apply(erule conjE)
+    subgoal premises prems3
+    apply(rule conjI)
+    apply(insert prems3(1,2))[1]
+      apply(rule weak_previous_LS5)
+      apply simp
+        apply(rule always_imp_refl)
+    apply(insert prems3(1,3))
+      apply(rule always_disj_rule)
+      apply simp
+        apply(erule conjE)
+        subgoal premises prems4
+        apply(rule conjI)
+        apply(insert prems4(1,2))[1]
+          apply(rule always_imp_refl)
+        apply(insert prems4(1,3))
+          apply(rule constrained_until_einv2req)
+          apply simp
+            apply(erule conjE)
+            subgoal premises prems5
+            apply(rule conjI)
+            apply(insert prems5(1,2))[1]
+              apply assumption
+            apply(insert prems5(1,3))
+              apply(erule conjE)
+              subgoal premises prems6
+              apply(rule conjI)
+              apply(insert prems6(1,2))[1]
+                apply assumption
+              apply(insert prems6(1,3))
+                apply assumption
+              done
+            done
+        done
+    done
+done
+done
+done
 
 lemma P1_2_inv_saving: "
 P1_2_inv_part t b_0 t1_0 A11 A12 A2 A3 s0 \<Longrightarrow>
 consecutive s0 s \<Longrightarrow>
 (((((t1_0 s0) = 0) \<or> (((A3 s) \<and> ((t1_0 s0) <= t)) \<or> ((A2 s) \<and> ((t1_0 s0) < (t1_0 s))))) \<and> ((b_0 s0) \<or> ((\<not> (A12 s)) \<or> ((A3 s) \<or> ((A2 s) \<and> ((t1_0 s) > 0)))))) \<and> ((b_0 s) --> (\<not> (A11 s)))) \<Longrightarrow>
-P1_2_inv_part t b_0 t1_0 A11 A12 A2 A3 s"
-  unfolding P1_2_inv_part_def
-  apply(simp add: P1_2_inv_saving_gen always_imp_refl)
-  done
+P1_2_inv_part t b_0 t1_0 A11 A12 A2 A3 s"unfolding P1_2_inv_part_def P1_2_part_def
+apply(simp add: P1_2_inv_saving_gen always_imp_refl)
+done
 
 lemma P1_2einv_imp_req: "
 P1_2_inv_part t b_0 t1_0 A11 A12 A2 A3 s \<Longrightarrow>
 toEnvP s \<Longrightarrow>
 ((t1_0 s) <= t) \<Longrightarrow>
-P1_2_part t A11 A12 A2 A3 s"
-  unfolding P1_2_inv_part_def P1_2_part_def
-  apply(simp add: P1_2einv_imp_req_gen always_imp_refl)
-  done
+P1_2_part t A11 A12 A2 A3 s"unfolding P1_2_inv_part_def P1_2_part_def
+apply(simp add: P1_2einv_imp_req_gen always_imp_refl)
+done
 
 lemmas P1_2_used_patterns = P1_2_def always_def weak_previous_def constrained_until_def 
 
@@ -167,8 +496,6 @@ lemmas P1_2_inv_part_used_patterns = P1_2_inv_part_def P1_2_inv_used_patterns
 
 lemmas P1_2_part_used_patterns = P1_2_part_def P1_2_used_patterns
 
-
-
 definition P2_1 where "P2_1 t A1 A2 s \<equiv> (always (\<lambda> r2 r1 . ((\<not> (A1 r1)) \<or> (constrained_always t A2 r2 r1))) s)"
 
 definition P2_1_part where "P2_1_part t A1 A2 s \<equiv> (P2_1 t A1 (\<lambda> s s1 . (A2 s1)) s)"
@@ -177,43 +504,110 @@ definition P2_1_inv where "P2_1_inv t t1_0 A1 A2_1 s \<equiv> (always_inv (\<lam
 
 definition P2_1_inv_part where "P2_1_inv_part t t1_0 A1 A2 s \<equiv> (P2_1_inv t t1_0 A1 (\<lambda> s s1 . (A2 s1)) s)"
 
-
-
 lemma P2_1_inv_saving_gen: "
 P2_1_inv t t1_0 A1 A2_1 s0 \<Longrightarrow>
 consecutive s0 s \<Longrightarrow>
 ((True \<and> ((t = 0) \<or> ((always_imp s0 (A2_1 s0) (A2_1 s)) \<and> (((((t1_0 s0) + 1) >= t) \<or> (A2_1 s s)) \<and> ((t1_0 s) <= ((t1_0 s0) + 1)))))) \<and> ((\<not> (A1 s)) \<or> ((t = 0) \<or> (((t1_0 s) = 0) \<and> (A2_1 s s))))) \<Longrightarrow>
 P2_1_inv t t1_0 A1 A2_1 s"
-  unfolding P2_1_inv_def
-  apply(proveOuter add_rules: invsaving)
+unfolding P2_1_inv_def
+apply(erule always_rule)
+  apply simp
+  apply(erule conjE)
+  subgoal premises prems1
+  apply(rule conjI)
+  apply(insert prems1(1,2))[1]
+    apply(rule always_disj_rule)
+    apply simp
+      apply(erule conjE)
+      subgoal premises prems2
+      apply(rule conjI)
+      apply(insert prems2(1,2))[1]
+        apply(rule always_imp_refl)
+      apply(insert prems2(1,3))
+        apply(rule constrained_always_rule)
+        apply simp
+          apply(erule disjE)
+          apply(rule disjI1)
+            apply assumption
+          apply(rule disjI2)
+            apply(erule conjE)
+            subgoal premises prems3
+            apply(rule conjI)
+            apply(insert prems3(1,2))[1]
+              apply assumption
+            apply(insert prems3(1,3))
+              apply(erule conjE)
+              subgoal premises prems4
+              apply(rule conjI)
+              apply(insert prems4(1,2))[1]
+                apply(erule disjE)
+                apply(rule disjI1)
+                  apply assumption
+                apply(rule disjI2)
+                  apply assumption
+              apply(insert prems4(1,3))
+                apply assumption
+              done
+            done
+      done
+  apply(insert prems1(1,3))
+    apply(erule disjE)
+    apply(rule disjI1)
+      apply assumption
+    apply(rule disjI2)
+      apply(rule constrained_always_one_point)
+      apply simp
+        apply(erule disjE)
+        apply(rule disjI1)
+          apply assumption
+        apply(rule disjI2)
+          apply(erule conjE)
+          subgoal premises prems5
+          apply(rule conjI)
+          apply(insert prems5(1,2))[1]
+            apply assumption
+          apply(insert prems5(1,3))
+            apply assumption
+          done
   done
+done
 
 lemma P2_1einv_imp_req_gen: "
 P2_1_inv t t1_0 A1 A2_1 s0 \<Longrightarrow>
 toEnvP s0 \<Longrightarrow>
 (True \<and> (always_imp s0 (A2_1 s0) (A2 s0))) \<Longrightarrow>
-P2_1 t A1 A2 s0"
-  unfolding P2_1_inv_def P2_1_def
-  apply(proveOuter add_rules: inv_req)
-  done
+P2_1 t A1 A2 s0"unfolding P2_1_inv_def P2_1_def
+apply(erule always_einv2req)
+apply simp
+  apply(rule always_disj_rule)
+  apply simp
+    apply(erule conjE)
+    subgoal premises prems3
+    apply(rule conjI)
+    apply(insert prems3(1,2))[1]
+      apply(rule always_imp_refl)
+    apply(insert prems3(1,3))
+      apply(rule constrained_always_einv2req)
+      apply simp
+        apply assumption
+    done
+done
 
 lemma P2_1_inv_saving: "
 P2_1_inv_part t t1_0 A1 A2 s0 \<Longrightarrow>
 consecutive s0 s \<Longrightarrow>
 (((t = 0) \<or> (((((t1_0 s0) + 1) >= t) \<or> (A2 s)) \<and> ((t1_0 s) <= ((t1_0 s0) + 1)))) \<and> ((\<not> (A1 s)) \<or> ((t = 0) \<or> (((t1_0 s) = 0) \<and> (A2 s))))) \<Longrightarrow>
-P2_1_inv_part t t1_0 A1 A2 s"
-  unfolding P2_1_inv_part_def
-  apply(simp add: P2_1_inv_saving_gen always_imp_refl)
-  done
+P2_1_inv_part t t1_0 A1 A2 s"unfolding P2_1_inv_part_def P2_1_part_def
+apply(simp add: P2_1_inv_saving_gen always_imp_refl)
+done
 
 lemma P2_1einv_imp_req: "
 P2_1_inv_part t t1_0 A1 A2 s \<Longrightarrow>
 toEnvP s \<Longrightarrow>
 True \<Longrightarrow>
-P2_1_part t A1 A2 s"
-  unfolding P2_1_inv_part_def P2_1_part_def
-  apply(simp add: P2_1einv_imp_req_gen always_imp_refl)
-  done
+P2_1_part t A1 A2 s"unfolding P2_1_inv_part_def P2_1_part_def
+apply(simp add: P2_1einv_imp_req_gen always_imp_refl)
+done
 
 lemmas P2_1_used_patterns = P2_1_def always_def constrained_always_def 
 
@@ -223,53 +617,176 @@ lemmas P2_1_inv_part_used_patterns = P2_1_inv_part_def P2_1_inv_used_patterns
 
 lemmas P2_1_part_used_patterns = P2_1_part_def P2_1_used_patterns
 
-
-
 definition P2_2 where "P2_2 t A11 A12 A2 s \<equiv> (always (\<lambda> r2 r1 . ((weak_previous (\<lambda> r4 r3 . (\<not> (A11 r3))) r2 r1) \<or> ((\<not> (A12 r1)) \<or> (constrained_always t A2 r2 r1)))) s)"
 
 definition P2_2_part where "P2_2_part t A11 A12 A2 s \<equiv> (P2_2 t A11 A12 (\<lambda> s s1 . (A2 s1)) s)"
 
-definition P2_2_inv where "P2_2_inv t b_0 t1_0 A11 A12 A2_1 s \<equiv> ((always_inv (\<lambda> r2 r1 . ((weak_previous (\<lambda> r4 r3 . (\<not> (A11 r3))) r2 r1) \<or> ((\<not> (A12 r1)) \<or> (constrained_always_inv t t1_0 A2_1 r2 r1)))) s) \<and> (b_0 s --> (previous_inv (\<lambda> r4 r3 . (\<not> (A11 r3))) s)))"
+definition P2_2_inv where "P2_2_inv t b_0 t1_0 A11 A12 A2_1 s \<equiv> ((always_inv (\<lambda> r2 r1 . ((weak_previous (\<lambda> r4 r3 . (\<not> (A11 r3))) r2 r1) \<or> ((\<not> (A12 r1)) \<or> (constrained_always_inv t t1_0 A2_1 r2 r1)))) s) \<and> (previous_inv b_0 (\<lambda> r4 r3 . (\<not> (A11 r3))) s))"
 
 definition P2_2_inv_part where "P2_2_inv_part t b_0 t1_0 A11 A12 A2 s \<equiv> (P2_2_inv t b_0 t1_0 A11 A12 (\<lambda> s s1 . (A2 s1)) s)"
-
-
 
 lemma P2_2_inv_saving_gen: "
 P2_2_inv t b_0 t1_0 A11 A12 A2_1 s0 \<Longrightarrow>
 consecutive s0 s \<Longrightarrow>
 (((True \<and> (True \<and> ((t = 0) \<or> ((always_imp s0 (A2_1 s0) (A2_1 s)) \<and> (((((t1_0 s0) + 1) >= t) \<or> (A2_1 s s)) \<and> ((t1_0 s) <= ((t1_0 s0) + 1))))))) \<and> (((b_0 s0) \<and> True) \<or> ((\<not> (A12 s)) \<or> ((t = 0) \<or> (((t1_0 s) = 0) \<and> (A2_1 s s)))))) \<and> ((b_0 s) --> (\<not> (A11 s)))) \<Longrightarrow>
 P2_2_inv t b_0 t1_0 A11 A12 A2_1 s"
-  unfolding P2_2_inv_def
-  apply(proveOuter add_rules: invsaving)
+unfolding P2_2_inv_def
+apply(erule conjE)
+apply(erule conjE)
+subgoal premises prems1
+apply(rule conjI)
+apply(insert prems1(1,2,4))[1]
+apply(erule always_rule)
+  apply simp
+  apply(erule conjE)
+  subgoal premises prems2
+  apply(rule conjI)
+  apply(insert prems2(1,2))[1]
+    apply(rule always_disj_rule)
+    apply simp
+      apply(erule conjE)
+      subgoal premises prems3
+      apply(rule conjI)
+      apply(insert prems3(1,2))[1]
+        apply(rule weak_previous_LS4)
+        apply simp
+          apply(rule always_imp_refl)
+      apply(insert prems3(1,3))
+        apply(rule always_disj_rule)
+        apply simp
+          apply(erule conjE)
+          subgoal premises prems4
+          apply(rule conjI)
+          apply(insert prems4(1,2))[1]
+            apply(rule always_imp_refl)
+          apply(insert prems4(1,3))
+            apply(rule constrained_always_rule)
+            apply simp
+              apply(erule disjE)
+              apply(rule disjI1)
+                apply assumption
+              apply(rule disjI2)
+                apply(erule conjE)
+                subgoal premises prems5
+                apply(rule conjI)
+                apply(insert prems5(1,2))[1]
+                  apply assumption
+                apply(insert prems5(1,3))
+                  apply(erule conjE)
+                  subgoal premises prems6
+                  apply(rule conjI)
+                  apply(insert prems6(1,2))[1]
+                    apply(erule disjE)
+                    apply(rule disjI1)
+                      apply assumption
+                    apply(rule disjI2)
+                      apply assumption
+                  apply(insert prems6(1,3))
+                    apply assumption
+                  done
+                done
+          done
+      done
+  apply(insert prems2(1,3))
+    apply(erule disjE)
+    apply(rule disjI1)
+      apply(rule weak_previous_one_point[OF prems1(3)])
+      apply simp
+        apply(erule conjE)
+        subgoal premises prems7
+        apply(rule conjI)
+        apply(insert prems7(1,2))[1]
+          apply assumption
+        apply(insert prems7(1,3))
+          apply(rule always_imp_refl)
+        done
+    apply(rule disjI2)
+      apply(erule disjE)
+      apply(rule disjI1)
+        apply assumption
+      apply(rule disjI2)
+        apply(rule constrained_always_one_point)
+        apply simp
+          apply(erule disjE)
+          apply(rule disjI1)
+            apply assumption
+          apply(rule disjI2)
+            apply(erule conjE)
+            subgoal premises prems8
+            apply(rule conjI)
+            apply(insert prems8(1,2))[1]
+              apply assumption
+            apply(insert prems8(1,3))
+              apply assumption
+            done
   done
+apply(insert prems1(1,3,5))
+  apply(erule previous_rule)
+  apply simp
+  apply(rule impI)
+  apply(erule impE)
+  apply assumption
+  subgoal premises prems9
+  apply(insert prems9(1,3))
+    apply assumption
+  done
+done
+done
 
 lemma P2_2einv_imp_req_gen: "
 P2_2_inv t b_0 t1_0 A11 A12 A2_1 s0 \<Longrightarrow>
 toEnvP s0 \<Longrightarrow>
 (True \<and> (True \<and> (always_imp s0 (A2_1 s0) (A2 s0)))) \<Longrightarrow>
-P2_2 t A11 A12 A2 s0"
-  unfolding P2_2_inv_def P2_2_def
-  apply(proveOuter add_rules: inv_req)
-  done
+P2_2 t A11 A12 A2 s0"unfolding P2_2_inv_def P2_2_def
+subgoal premises prems1
+apply(insert prems1(1,2))
+apply(erule conjE)
+subgoal premises prems2
+apply(insert prems2(1,2) prems1(3))
+apply(erule always_einv2req)
+apply simp
+  apply(rule always_disj_rule)
+  apply simp
+    apply(erule conjE)
+    subgoal premises prems3
+    apply(rule conjI)
+    apply(insert prems3(1,2))[1]
+      apply(rule weak_previous_LS5)
+      apply simp
+        apply(rule always_imp_refl)
+    apply(insert prems3(1,3))
+      apply(rule always_disj_rule)
+      apply simp
+        apply(erule conjE)
+        subgoal premises prems4
+        apply(rule conjI)
+        apply(insert prems4(1,2))[1]
+          apply(rule always_imp_refl)
+        apply(insert prems4(1,3))
+          apply(rule constrained_always_einv2req)
+          apply simp
+            apply assumption
+        done
+    done
+done
+done
+done
 
 lemma P2_2_inv_saving: "
 P2_2_inv_part t b_0 t1_0 A11 A12 A2 s0 \<Longrightarrow>
 consecutive s0 s \<Longrightarrow>
 ((((t = 0) \<or> (((((t1_0 s0) + 1) >= t) \<or> (A2 s)) \<and> ((t1_0 s) <= ((t1_0 s0) + 1)))) \<and> ((b_0 s0) \<or> ((\<not> (A12 s)) \<or> ((t = 0) \<or> (((t1_0 s) = 0) \<and> (A2 s)))))) \<and> ((b_0 s) --> (\<not> (A11 s)))) \<Longrightarrow>
-P2_2_inv_part t b_0 t1_0 A11 A12 A2 s"
-  unfolding P2_2_inv_part_def
-  apply(simp add: P2_2_inv_saving_gen always_imp_refl)
-  done
+P2_2_inv_part t b_0 t1_0 A11 A12 A2 s"unfolding P2_2_inv_part_def P2_2_part_def
+apply(simp add: P2_2_inv_saving_gen always_imp_refl)
+done
 
 lemma P2_2einv_imp_req: "
 P2_2_inv_part t b_0 t1_0 A11 A12 A2 s \<Longrightarrow>
 toEnvP s \<Longrightarrow>
 True \<Longrightarrow>
-P2_2_part t A11 A12 A2 s"
-  unfolding P2_2_inv_part_def P2_2_part_def
-  apply(simp add: P2_2einv_imp_req_gen always_imp_refl)
-  done
+P2_2_part t A11 A12 A2 s"unfolding P2_2_inv_part_def P2_2_part_def
+apply(simp add: P2_2einv_imp_req_gen always_imp_refl)
+done
 
 lemmas P2_2_used_patterns = P2_2_def always_def weak_previous_def constrained_always_def 
 
@@ -279,8 +796,6 @@ lemmas P2_2_inv_part_used_patterns = P2_2_inv_part_def P2_2_inv_used_patterns
 
 lemmas P2_2_part_used_patterns = P2_2_part_def P2_2_used_patterns
 
-
-
 definition P3_1 where "P3_1 A1 A2 A3 s \<equiv> (always (\<lambda> r2 r1 . ((\<not> (A1 r1)) \<or> (weak_until A2 A3 r2 r1))) s)"
 
 definition P3_1_part where "P3_1_part A1 A2 A3 s \<equiv> (P3_1 A1 (\<lambda> s s1 . (A2 s1)) (\<lambda> s s1 . (A3 s1)) s)"
@@ -289,43 +804,124 @@ definition P3_1_inv where "P3_1_inv w_0 A1 A2_1 A3_1 s \<equiv> (always_inv (\<l
 
 definition P3_1_inv_part where "P3_1_inv_part w_0 A1 A2 A3 s \<equiv> (P3_1_inv w_0 A1 (\<lambda> s s1 . (A2 s1)) (\<lambda> s s1 . (A3 s1)) s)"
 
-
-
 lemma P3_1_inv_saving_gen: "
 P3_1_inv w_0 A1 A2_1 A3_1 s0 \<Longrightarrow>
 consecutive s0 s \<Longrightarrow>
 ((True \<and> ((always_imp s0 (A2_1 s0) (A2_1 s)) \<and> ((always_imp s0 (A3_1 s0) (A3_1 s)) \<and> ((\<not> (w_0 s0)) \<or> ((A3_1 s s) \<or> ((w_0 s) \<and> (A2_1 s s))))))) \<and> ((\<not> (A1 s)) \<or> ((A3_1 s s) \<or> ((w_0 s) \<and> (A2_1 s s))))) \<Longrightarrow>
 P3_1_inv w_0 A1 A2_1 A3_1 s"
-  unfolding P3_1_inv_def
-  apply(proveOuter add_rules: invsaving)
+unfolding P3_1_inv_def
+apply(erule always_rule)
+  apply simp
+  apply(erule conjE)
+  subgoal premises prems1
+  apply(rule conjI)
+  apply(insert prems1(1,2))[1]
+    apply(rule always_disj_rule)
+    apply simp
+      apply(erule conjE)
+      subgoal premises prems2
+      apply(rule conjI)
+      apply(insert prems2(1,2))[1]
+        apply(rule always_imp_refl)
+      apply(insert prems2(1,3))
+        apply(rule weak_until_rule)
+        apply simp
+          apply(erule conjE)
+          subgoal premises prems3
+          apply(rule conjI)
+          apply(insert prems3(1,2))[1]
+            apply assumption
+          apply(insert prems3(1,3))
+            apply(erule conjE)
+            subgoal premises prems4
+            apply(rule conjI)
+            apply(insert prems4(1,2))[1]
+              apply assumption
+            apply(insert prems4(1,3))
+              apply(erule disjE)
+              apply(rule disjI1)
+                apply assumption
+              apply(rule disjI2)
+                apply(erule disjE)
+                apply(rule disjI1)
+                  apply assumption
+                apply(rule disjI2)
+                  apply(erule conjE)
+                  subgoal premises prems5
+                  apply(rule conjI)
+                  apply(insert prems5(1,2))[1]
+                    apply assumption
+                  apply(insert prems5(1,3))
+                    apply assumption
+                  done
+            done
+          done
+      done
+  apply(insert prems1(1,3))
+    apply(erule disjE)
+    apply(rule disjI1)
+      apply assumption
+    apply(rule disjI2)
+      apply(rule weak_until_one_point)
+      apply simp
+        apply(erule disjE)
+        apply(rule disjI1)
+          apply assumption
+        apply(rule disjI2)
+          apply(erule conjE)
+          subgoal premises prems6
+          apply(rule conjI)
+          apply(insert prems6(1,2))[1]
+            apply assumption
+          apply(insert prems6(1,3))
+            apply assumption
+          done
   done
+done
 
 lemma P3_1einv_imp_req_gen: "
 P3_1_inv w_0 A1 A2_1 A3_1 s0 \<Longrightarrow>
 toEnvP s0 \<Longrightarrow>
 (True \<and> ((always_imp s0 (A2_1 s0) (A2 s0)) \<and> (always_imp s0 (A3_1 s0) (A3 s0)))) \<Longrightarrow>
-P3_1 A1 A2 A3 s0"
-  unfolding P3_1_inv_def P3_1_def
-  apply(proveOuter add_rules: inv_req)
-  done
+P3_1 A1 A2 A3 s0"unfolding P3_1_inv_def P3_1_def
+apply(erule always_einv2req)
+apply simp
+  apply(rule always_disj_rule)
+  apply simp
+    apply(erule conjE)
+    subgoal premises prems3
+    apply(rule conjI)
+    apply(insert prems3(1,2))[1]
+      apply(rule always_imp_refl)
+    apply(insert prems3(1,3))
+      apply(rule weak_until_einv2req)
+      apply simp
+        apply(erule conjE)
+        subgoal premises prems4
+        apply(rule conjI)
+        apply(insert prems4(1,2))[1]
+          apply assumption
+        apply(insert prems4(1,3))
+          apply assumption
+        done
+    done
+done
 
 lemma P3_1_inv_saving: "
 P3_1_inv_part w_0 A1 A2 A3 s0 \<Longrightarrow>
 consecutive s0 s \<Longrightarrow>
 (((\<not> (w_0 s0)) \<or> ((A3 s) \<or> ((w_0 s) \<and> (A2 s)))) \<and> ((\<not> (A1 s)) \<or> ((A3 s) \<or> ((w_0 s) \<and> (A2 s))))) \<Longrightarrow>
-P3_1_inv_part w_0 A1 A2 A3 s"
-  unfolding P3_1_inv_part_def
-  apply(simp add: P3_1_inv_saving_gen always_imp_refl)
-  done
+P3_1_inv_part w_0 A1 A2 A3 s"unfolding P3_1_inv_part_def P3_1_part_def
+apply(simp add: P3_1_inv_saving_gen always_imp_refl)
+done
 
 lemma P3_1einv_imp_req: "
 P3_1_inv_part w_0 A1 A2 A3 s \<Longrightarrow>
 toEnvP s \<Longrightarrow>
 True \<Longrightarrow>
-P3_1_part A1 A2 A3 s"
-  unfolding P3_1_inv_part_def P3_1_part_def
-  apply(simp add: P3_1einv_imp_req_gen always_imp_refl)
-  done
+P3_1_part A1 A2 A3 s"unfolding P3_1_inv_part_def P3_1_part_def
+apply(simp add: P3_1einv_imp_req_gen always_imp_refl)
+done
 
 lemmas P3_1_used_patterns = P3_1_def always_def weak_until_def 
 
@@ -335,51 +931,190 @@ lemmas P3_1_inv_part_used_patterns = P3_1_inv_part_def P3_1_inv_used_patterns
 
 lemmas P3_1_part_used_patterns = P3_1_part_def P3_1_used_patterns
 
-
-
 definition P3_2 where "P3_2 A11 A12 A2 A3 s \<equiv> (always (\<lambda> r2 r1 . ((weak_previous (\<lambda> r4 r3 . (\<not> (A11 r3))) r2 r1) \<or> ((\<not> (A12 r1)) \<or> (weak_until A2 A3 r2 r1)))) s)"
 
 definition P3_2_part where "P3_2_part A11 A12 A2 A3 s \<equiv> (P3_2 A11 A12 (\<lambda> s s1 . (A2 s1)) (\<lambda> s s1 . (A3 s1)) s)"
 
-definition P3_2_inv where "P3_2_inv b_0 w_0 A11 A12 A2_1 A3_1 s \<equiv> ((always_inv (\<lambda> r2 r1 . ((weak_previous (\<lambda> r4 r3 . (\<not> (A11 r3))) r2 r1) \<or> ((\<not> (A12 r1)) \<or> (weak_until_inv w_0 A2_1 A3_1 r2 r1)))) s) \<and> (b_0 s --> (previous_inv (\<lambda> r4 r3 . (\<not> (A11 r3))) s)))"
+definition P3_2_inv where "P3_2_inv b_0 w_0 A11 A12 A2_1 A3_1 s \<equiv> ((always_inv (\<lambda> r2 r1 . ((weak_previous (\<lambda> r4 r3 . (\<not> (A11 r3))) r2 r1) \<or> ((\<not> (A12 r1)) \<or> (weak_until_inv w_0 A2_1 A3_1 r2 r1)))) s) \<and> (previous_inv b_0 (\<lambda> r4 r3 . (\<not> (A11 r3))) s))"
 
 definition P3_2_inv_part where "P3_2_inv_part b_0 w_0 A11 A12 A2 A3 s \<equiv> (P3_2_inv b_0 w_0 A11 A12 (\<lambda> s s1 . (A2 s1)) (\<lambda> s s1 . (A3 s1)) s)"
-
-
 
 lemma P3_2_inv_saving_gen: "
 P3_2_inv b_0 w_0 A11 A12 A2_1 A3_1 s0 \<Longrightarrow>
 consecutive s0 s \<Longrightarrow>
 (((True \<and> (True \<and> ((always_imp s0 (A2_1 s0) (A2_1 s)) \<and> ((always_imp s0 (A3_1 s0) (A3_1 s)) \<and> ((\<not> (w_0 s0)) \<or> ((A3_1 s s) \<or> ((w_0 s) \<and> (A2_1 s s)))))))) \<and> (((b_0 s0) \<and> True) \<or> ((\<not> (A12 s)) \<or> ((A3_1 s s) \<or> ((w_0 s) \<and> (A2_1 s s)))))) \<and> ((b_0 s) --> (\<not> (A11 s)))) \<Longrightarrow>
 P3_2_inv b_0 w_0 A11 A12 A2_1 A3_1 s"
-  unfolding P3_2_inv_def P3_2_def
-  apply(proveOuter add_rules: invsaving)
+unfolding P3_2_inv_def
+apply(erule conjE)
+apply(erule conjE)
+subgoal premises prems1
+apply(rule conjI)
+apply(insert prems1(1,2,4))[1]
+apply(erule always_rule)
+  apply simp
+  apply(erule conjE)
+  subgoal premises prems2
+  apply(rule conjI)
+  apply(insert prems2(1,2))[1]
+    apply(rule always_disj_rule)
+    apply simp
+      apply(erule conjE)
+      subgoal premises prems3
+      apply(rule conjI)
+      apply(insert prems3(1,2))[1]
+        apply(rule weak_previous_LS4)
+        apply simp
+          apply(rule always_imp_refl)
+      apply(insert prems3(1,3))
+        apply(rule always_disj_rule)
+        apply simp
+          apply(erule conjE)
+          subgoal premises prems4
+          apply(rule conjI)
+          apply(insert prems4(1,2))[1]
+            apply(rule always_imp_refl)
+          apply(insert prems4(1,3))
+            apply(rule weak_until_rule)
+            apply simp
+              apply(erule conjE)
+              subgoal premises prems5
+              apply(rule conjI)
+              apply(insert prems5(1,2))[1]
+                apply assumption
+              apply(insert prems5(1,3))
+                apply(erule conjE)
+                subgoal premises prems6
+                apply(rule conjI)
+                apply(insert prems6(1,2))[1]
+                  apply assumption
+                apply(insert prems6(1,3))
+                  apply(erule disjE)
+                  apply(rule disjI1)
+                    apply assumption
+                  apply(rule disjI2)
+                    apply(erule disjE)
+                    apply(rule disjI1)
+                      apply assumption
+                    apply(rule disjI2)
+                      apply(erule conjE)
+                      subgoal premises prems7
+                      apply(rule conjI)
+                      apply(insert prems7(1,2))[1]
+                        apply assumption
+                      apply(insert prems7(1,3))
+                        apply assumption
+                      done
+                done
+              done
+          done
+      done
+  apply(insert prems2(1,3))
+    apply(erule disjE)
+    apply(rule disjI1)
+      apply(rule weak_previous_one_point[OF prems1(3)])
+      apply simp
+        apply(erule conjE)
+        subgoal premises prems8
+        apply(rule conjI)
+        apply(insert prems8(1,2))[1]
+          apply assumption
+        apply(insert prems8(1,3))
+          apply(rule always_imp_refl)
+        done
+    apply(rule disjI2)
+      apply(erule disjE)
+      apply(rule disjI1)
+        apply assumption
+      apply(rule disjI2)
+        apply(rule weak_until_one_point)
+        apply simp
+          apply(erule disjE)
+          apply(rule disjI1)
+            apply assumption
+          apply(rule disjI2)
+            apply(erule conjE)
+            subgoal premises prems9
+            apply(rule conjI)
+            apply(insert prems9(1,2))[1]
+              apply assumption
+            apply(insert prems9(1,3))
+              apply assumption
+            done
   done
+apply(insert prems1(1,3,5))
+  apply(erule previous_rule)
+  apply simp
+  apply(rule impI)
+  apply(erule impE)
+  apply assumption
+  subgoal premises prems10
+  apply(insert prems10(1,3))
+    apply assumption
+  done
+done
+done
 
 lemma P3_2einv_imp_req_gen: "
 P3_2_inv b_0 w_0 A11 A12 A2_1 A3_1 s0 \<Longrightarrow>
 toEnvP s0 \<Longrightarrow>
 (True \<and> (True \<and> ((always_imp s0 (A2_1 s0) (A2 s0)) \<and> (always_imp s0 (A3_1 s0) (A3 s0))))) \<Longrightarrow>
-P3_2 A11 A12 A2 A3 s0"
-  unfolding P3_2_inv_def P3_2_def
-  apply(proveOuter add_rules: inv_req)
-  done
+P3_2 A11 A12 A2 A3 s0"unfolding P3_2_inv_def P3_2_def
+subgoal premises prems1
+apply(insert prems1(1,2))
+apply(erule conjE)
+subgoal premises prems2
+apply(insert prems2(1,2) prems1(3))
+apply(erule always_einv2req)
+apply simp
+  apply(rule always_disj_rule)
+  apply simp
+    apply(erule conjE)
+    subgoal premises prems3
+    apply(rule conjI)
+    apply(insert prems3(1,2))[1]
+      apply(rule weak_previous_LS5)
+      apply simp
+        apply(rule always_imp_refl)
+    apply(insert prems3(1,3))
+      apply(rule always_disj_rule)
+      apply simp
+        apply(erule conjE)
+        subgoal premises prems4
+        apply(rule conjI)
+        apply(insert prems4(1,2))[1]
+          apply(rule always_imp_refl)
+        apply(insert prems4(1,3))
+          apply(rule weak_until_einv2req)
+          apply simp
+            apply(erule conjE)
+            subgoal premises prems5
+            apply(rule conjI)
+            apply(insert prems5(1,2))[1]
+              apply assumption
+            apply(insert prems5(1,3))
+              apply assumption
+            done
+        done
+    done
+done
+done
+done
 
 lemma P3_2_inv_saving: "
 P3_2_inv_part b_0 w_0 A11 A12 A2 A3 s0 \<Longrightarrow>
 consecutive s0 s \<Longrightarrow>
 ((((\<not> (w_0 s0)) \<or> ((A3 s) \<or> ((w_0 s) \<and> (A2 s)))) \<and> ((b_0 s0) \<or> ((\<not> (A12 s)) \<or> ((A3 s) \<or> ((w_0 s) \<and> (A2 s)))))) \<and> ((b_0 s) --> (\<not> (A11 s)))) \<Longrightarrow>
-P3_2_inv_part b_0 w_0 A11 A12 A2 A3 s"
-  unfolding P3_2_inv_part_def
-  by(simp add: P3_2_inv_saving_gen always_imp_refl)
+P3_2_inv_part b_0 w_0 A11 A12 A2 A3 s"unfolding P3_2_inv_part_def P3_2_part_def
+apply(simp add: P3_2_inv_saving_gen always_imp_refl)
+done
 
 lemma P3_2einv_imp_req: "
 P3_2_inv_part b_0 w_0 A11 A12 A2 A3 s \<Longrightarrow>
 toEnvP s \<Longrightarrow>
 True \<Longrightarrow>
-P3_2_part A11 A12 A2 A3 s"
-  unfolding P3_2_inv_part_def P3_2_part_def
-  by(simp add: P3_2einv_imp_req_gen always_imp_refl)
+P3_2_part A11 A12 A2 A3 s"unfolding P3_2_inv_part_def P3_2_part_def
+apply(simp add: P3_2einv_imp_req_gen always_imp_refl)
+done
 
 lemmas P3_2_used_patterns = P3_2_def always_def weak_previous_def weak_until_def 
 
@@ -389,51 +1124,168 @@ lemmas P3_2_inv_part_used_patterns = P3_2_inv_part_def P3_2_inv_used_patterns
 
 lemmas P3_2_part_used_patterns = P3_2_part_def P3_2_used_patterns
 
-
-
 definition P3_3 where "P3_3 A1 A2 A3 s \<equiv> (always (\<lambda> r2 r1 . ((weak_previous (\<lambda> r4 r3 . (\<not> (A1 r3))) r2 r1) \<or> (weak_until A2 A3 r2 r1))) s)"
 
 definition P3_3_part where "P3_3_part A1 A2 A3 s \<equiv> (P3_3 A1 (\<lambda> s s1 . (A2 s1)) (\<lambda> s s1 . (A3 s1)) s)"
 
-definition P3_3_inv where "P3_3_inv b_0 w_0 A1 A2_1 A3_1 s \<equiv> ((always_inv (\<lambda> r2 r1 . ((weak_previous (\<lambda> r4 r3 . (\<not> (A1 r3))) r2 r1) \<or> (weak_until_inv w_0 A2_1 A3_1 r2 r1))) s) \<and> (b_0 s --> (previous_inv (\<lambda> r4 r3 . (\<not> (A1 r3))) s)))"
+definition P3_3_inv where "P3_3_inv b_0 w_0 A1 A2_1 A3_1 s \<equiv> ((always_inv (\<lambda> r2 r1 . ((weak_previous (\<lambda> r4 r3 . (\<not> (A1 r3))) r2 r1) \<or> (weak_until_inv w_0 A2_1 A3_1 r2 r1))) s) \<and> (previous_inv b_0 (\<lambda> r4 r3 . (\<not> (A1 r3))) s))"
 
 definition P3_3_inv_part where "P3_3_inv_part b_0 w_0 A1 A2 A3 s \<equiv> (P3_3_inv b_0 w_0 A1 (\<lambda> s s1 . (A2 s1)) (\<lambda> s s1 . (A3 s1)) s)"
-
-
 
 lemma P3_3_inv_saving_gen: "
 P3_3_inv b_0 w_0 A1 A2_1 A3_1 s0 \<Longrightarrow>
 consecutive s0 s \<Longrightarrow>
 (((True \<and> ((always_imp s0 (A2_1 s0) (A2_1 s)) \<and> ((always_imp s0 (A3_1 s0) (A3_1 s)) \<and> ((\<not> (w_0 s0)) \<or> ((A3_1 s s) \<or> ((w_0 s) \<and> (A2_1 s s))))))) \<and> (((b_0 s0) \<and> True) \<or> ((A3_1 s s) \<or> ((w_0 s) \<and> (A2_1 s s))))) \<and> ((b_0 s) --> (\<not> (A1 s)))) \<Longrightarrow>
 P3_3_inv b_0 w_0 A1 A2_1 A3_1 s"
-  unfolding P3_3_inv_def  P3_3_def
-  apply(proveOuter add_rules: invsaving)
+unfolding P3_3_inv_def
+apply(erule conjE)
+apply(erule conjE)
+subgoal premises prems1
+apply(rule conjI)
+apply(insert prems1(1,2,4))[1]
+apply(erule always_rule)
+  apply simp
+  apply(erule conjE)
+  subgoal premises prems2
+  apply(rule conjI)
+  apply(insert prems2(1,2))[1]
+    apply(rule always_disj_rule)
+    apply simp
+      apply(erule conjE)
+      subgoal premises prems3
+      apply(rule conjI)
+      apply(insert prems3(1,2))[1]
+        apply(rule weak_previous_LS4)
+        apply simp
+          apply(rule always_imp_refl)
+      apply(insert prems3(1,3))
+        apply(rule weak_until_rule)
+        apply simp
+          apply(erule conjE)
+          subgoal premises prems4
+          apply(rule conjI)
+          apply(insert prems4(1,2))[1]
+            apply assumption
+          apply(insert prems4(1,3))
+            apply(erule conjE)
+            subgoal premises prems5
+            apply(rule conjI)
+            apply(insert prems5(1,2))[1]
+              apply assumption
+            apply(insert prems5(1,3))
+              apply(erule disjE)
+              apply(rule disjI1)
+                apply assumption
+              apply(rule disjI2)
+                apply(erule disjE)
+                apply(rule disjI1)
+                  apply assumption
+                apply(rule disjI2)
+                  apply(erule conjE)
+                  subgoal premises prems6
+                  apply(rule conjI)
+                  apply(insert prems6(1,2))[1]
+                    apply assumption
+                  apply(insert prems6(1,3))
+                    apply assumption
+                  done
+            done
+          done
+      done
+  apply(insert prems2(1,3))
+    apply(erule disjE)
+    apply(rule disjI1)
+      apply(rule weak_previous_one_point[OF prems1(3)])
+      apply simp
+        apply(erule conjE)
+        subgoal premises prems7
+        apply(rule conjI)
+        apply(insert prems7(1,2))[1]
+          apply assumption
+        apply(insert prems7(1,3))
+          apply(rule always_imp_refl)
+        done
+    apply(rule disjI2)
+      apply(rule weak_until_one_point)
+      apply simp
+        apply(erule disjE)
+        apply(rule disjI1)
+          apply assumption
+        apply(rule disjI2)
+          apply(erule conjE)
+          subgoal premises prems8
+          apply(rule conjI)
+          apply(insert prems8(1,2))[1]
+            apply assumption
+          apply(insert prems8(1,3))
+            apply assumption
+          done
   done
+apply(insert prems1(1,3,5))
+  apply(erule previous_rule)
+  apply simp
+  apply(rule impI)
+  apply(erule impE)
+  apply assumption
+  subgoal premises prems9
+  apply(insert prems9(1,3))
+    apply assumption
+  done
+done
+done
 
 lemma P3_3einv_imp_req_gen: "
 P3_3_inv b_0 w_0 A1 A2_1 A3_1 s0 \<Longrightarrow>
 toEnvP s0 \<Longrightarrow>
 (True \<and> ((always_imp s0 (A2_1 s0) (A2 s0)) \<and> (always_imp s0 (A3_1 s0) (A3 s0)))) \<Longrightarrow>
-P3_3 A1 A2 A3 s0"
-  unfolding P3_3_inv_def  P3_3_def
-  apply(proveOuter add_rules: inv_req)
-  done
+P3_3 A1 A2 A3 s0"unfolding P3_3_inv_def P3_3_def
+subgoal premises prems1
+apply(insert prems1(1,2))
+apply(erule conjE)
+subgoal premises prems2
+apply(insert prems2(1,2) prems1(3))
+apply(erule always_einv2req)
+apply simp
+  apply(rule always_disj_rule)
+  apply simp
+    apply(erule conjE)
+    subgoal premises prems3
+    apply(rule conjI)
+    apply(insert prems3(1,2))[1]
+      apply(rule weak_previous_LS5)
+      apply simp
+        apply(rule always_imp_refl)
+    apply(insert prems3(1,3))
+      apply(rule weak_until_einv2req)
+      apply simp
+        apply(erule conjE)
+        subgoal premises prems4
+        apply(rule conjI)
+        apply(insert prems4(1,2))[1]
+          apply assumption
+        apply(insert prems4(1,3))
+          apply assumption
+        done
+    done
+done
+done
+done
 
 lemma P3_3_inv_saving: "
 P3_3_inv_part b_0 w_0 A1 A2 A3 s0 \<Longrightarrow>
 consecutive s0 s \<Longrightarrow>
 ((((\<not> (w_0 s0)) \<or> ((A3 s) \<or> ((w_0 s) \<and> (A2 s)))) \<and> ((b_0 s0) \<or> ((A3 s) \<or> ((w_0 s) \<and> (A2 s))))) \<and> ((b_0 s) --> (\<not> (A1 s)))) \<Longrightarrow>
-P3_3_inv_part b_0 w_0 A1 A2 A3 s"
-  unfolding P3_3_inv_part_def
-  by(simp add: P3_3_inv_saving_gen always_imp_refl)
+P3_3_inv_part b_0 w_0 A1 A2 A3 s"unfolding P3_3_inv_part_def P3_3_part_def
+apply(simp add: P3_3_inv_saving_gen always_imp_refl)
+done
 
 lemma P3_3einv_imp_req: "
 P3_3_inv_part b_0 w_0 A1 A2 A3 s \<Longrightarrow>
 toEnvP s \<Longrightarrow>
 True \<Longrightarrow>
-P3_3_part A1 A2 A3 s"
-  unfolding P3_3_inv_part_def P3_3_part_def
-  by(simp add: P3_3einv_imp_req_gen always_imp_refl)
+P3_3_part A1 A2 A3 s"unfolding P3_3_inv_part_def P3_3_part_def
+apply(simp add: P3_3einv_imp_req_gen always_imp_refl)
+done
 
 lemmas P3_3_used_patterns = P3_3_def always_def weak_previous_def weak_until_def 
 
@@ -443,51 +1295,231 @@ lemmas P3_3_inv_part_used_patterns = P3_3_inv_part_def P3_3_inv_used_patterns
 
 lemmas P3_3_part_used_patterns = P3_3_part_def P3_3_used_patterns
 
-
-
 definition P3_4 where "P3_4 A11 A12 A2 A3 s \<equiv> (always (\<lambda> r2 r1 . ((weak_previous (\<lambda> r4 r3 . ((weak_previous (\<lambda> r6 r5 . (\<not> (A11 r5))) r4 r3) \<or> (\<not> (A12 r3)))) r2 r1) \<or> (weak_until A2 A3 r2 r1))) s)"
 
 definition P3_4_part where "P3_4_part A11 A12 A2 A3 s \<equiv> (P3_4 A11 A12 (\<lambda> s s1 . (A2 s1)) (\<lambda> s s1 . (A3 s1)) s)"
 
-definition P3_4_inv where "P3_4_inv b_0 b_1 w_0 A11 A12 A2_1 A3_1 s \<equiv> (((always_inv (\<lambda> r2 r1 . ((weak_previous (\<lambda> r4 r3 . ((weak_previous (\<lambda> r6 r5 . (\<not> (A11 r5))) r4 r3) \<or> (\<not> (A12 r3)))) r2 r1) \<or> (weak_until_inv w_0 A2_1 A3_1 r2 r1))) s) \<and> (b_1 s --> (previous_inv (\<lambda> r4 r3 . ((weak_previous (\<lambda> r6 r5 . (\<not> (A11 r5))) r4 r3) \<or> (\<not> (A12 r3)))) s))) \<and> (b_0 s --> (previous_inv (\<lambda> r6 r5 . (\<not> (A11 r5))) s)))"
+definition P3_4_inv where "P3_4_inv b_0 b_1 w_0 A11 A12 A2_1 A3_1 s \<equiv> (((always_inv (\<lambda> r2 r1 . ((weak_previous (\<lambda> r4 r3 . ((weak_previous (\<lambda> r6 r5 . (\<not> (A11 r5))) r4 r3) \<or> (\<not> (A12 r3)))) r2 r1) \<or> (weak_until_inv w_0 A2_1 A3_1 r2 r1))) s) \<and> (previous_inv b_1 (\<lambda> r4 r3 . ((weak_previous (\<lambda> r6 r5 . (\<not> (A11 r5))) r4 r3) \<or> (\<not> (A12 r3)))) s)) \<and> (previous_inv b_0 (\<lambda> r6 r5 . (\<not> (A11 r5))) s))"
 
 definition P3_4_inv_part where "P3_4_inv_part b_0 b_1 w_0 A11 A12 A2 A3 s \<equiv> (P3_4_inv b_0 b_1 w_0 A11 A12 (\<lambda> s s1 . (A2 s1)) (\<lambda> s s1 . (A3 s1)) s)"
-
-
 
 lemma P3_4_inv_saving_gen: "
 P3_4_inv b_0 b_1 w_0 A11 A12 A2_1 A3_1 s0 \<Longrightarrow>
 consecutive s0 s \<Longrightarrow>
 (((((True \<and> True) \<and> ((always_imp s0 (A2_1 s0) (A2_1 s)) \<and> ((always_imp s0 (A3_1 s0) (A3_1 s)) \<and> ((\<not> (w_0 s0)) \<or> ((A3_1 s s) \<or> ((w_0 s) \<and> (A2_1 s s))))))) \<and> (((b_1 s0) \<and> (True \<and> True)) \<or> ((A3_1 s s) \<or> ((w_0 s) \<and> (A2_1 s s))))) \<and> ((b_1 s) --> (((b_0 s0) \<and> True) \<or> (\<not> (A12 s))))) \<and> ((b_0 s) --> (\<not> (A11 s)))) \<Longrightarrow>
 P3_4_inv b_0 b_1 w_0 A11 A12 A2_1 A3_1 s"
-  unfolding P3_4_inv_def P3_4_def
-  apply(proveOuter add_rules: invsaving)
+unfolding P3_4_inv_def
+apply(erule conjE)
+apply(erule conjE)
+subgoal premises prems1
+apply(rule conjI)
+apply(insert prems1(1,2,4))[1]
+apply(erule conjE)
+apply(erule conjE)
+subgoal premises prems2
+apply(rule conjI)
+apply(insert prems2(1,2,4))[1]
+apply(erule always_rule)
+  apply simp
+  apply(erule conjE)
+  subgoal premises prems3
+  apply(rule conjI)
+  apply(insert prems3(1,2))[1]
+    apply(rule always_disj_rule)
+    apply simp
+      apply(erule conjE)
+      subgoal premises prems4
+      apply(rule conjI)
+      apply(insert prems4(1,2))[1]
+        apply(rule weak_previous_LS4)
+        apply simp
+          apply(rule always_disj_rule)
+          apply simp
+            apply(erule conjE)
+            subgoal premises prems5
+            apply(rule conjI)
+            apply(insert prems5(1,2))[1]
+              apply(rule weak_previous_LS4)
+              apply simp
+                apply(rule always_imp_refl)
+            apply(insert prems5(1,3))
+              apply(rule always_imp_refl)
+            done
+      apply(insert prems4(1,3))
+        apply(rule weak_until_rule)
+        apply simp
+          apply(erule conjE)
+          subgoal premises prems6
+          apply(rule conjI)
+          apply(insert prems6(1,2))[1]
+            apply assumption
+          apply(insert prems6(1,3))
+            apply(erule conjE)
+            subgoal premises prems7
+            apply(rule conjI)
+            apply(insert prems7(1,2))[1]
+              apply assumption
+            apply(insert prems7(1,3))
+              apply(erule disjE)
+              apply(rule disjI1)
+                apply assumption
+              apply(rule disjI2)
+                apply(erule disjE)
+                apply(rule disjI1)
+                  apply assumption
+                apply(rule disjI2)
+                  apply(erule conjE)
+                  subgoal premises prems8
+                  apply(rule conjI)
+                  apply(insert prems8(1,2))[1]
+                    apply assumption
+                  apply(insert prems8(1,3))
+                    apply assumption
+                  done
+            done
+          done
+      done
+  apply(insert prems3(1,3))
+    apply(erule disjE)
+    apply(rule disjI1)
+      apply(rule weak_previous_one_point[OF prems2(3)])
+      apply simp
+        apply(erule conjE)
+        subgoal premises prems9
+        apply(rule conjI)
+        apply(insert prems9(1,2))[1]
+          apply assumption
+        apply(insert prems9(1,3))
+          apply(rule always_disj_rule)
+          apply simp
+            apply(erule conjE)
+            subgoal premises prems10
+            apply(rule conjI)
+            apply(insert prems10(1,2))[1]
+              apply(rule weak_previous_LS4)
+              apply simp
+                apply(rule always_imp_refl)
+            apply(insert prems10(1,3))
+              apply(rule always_imp_refl)
+            done
+        done
+    apply(rule disjI2)
+      apply(rule weak_until_one_point)
+      apply simp
+        apply(erule disjE)
+        apply(rule disjI1)
+          apply assumption
+        apply(rule disjI2)
+          apply(erule conjE)
+          subgoal premises prems11
+          apply(rule conjI)
+          apply(insert prems11(1,2))[1]
+            apply assumption
+          apply(insert prems11(1,3))
+            apply assumption
+          done
   done
+apply(insert prems2(1,3,5))
+  apply(erule previous_rule)
+  apply simp
+  apply(rule impI)
+  apply(erule impE)
+  apply assumption
+  subgoal premises prems12
+  apply(insert prems12(1,3))
+    apply(erule disjE)
+    apply(rule disjI1)
+      apply(rule weak_previous_one_point[OF prems1(3)])
+      apply simp
+        apply(erule conjE)
+        subgoal premises prems13
+        apply(rule conjI)
+        apply(insert prems13(1,2))[1]
+          apply assumption
+        apply(insert prems13(1,3))
+          apply(rule always_imp_refl)
+        done
+    apply(rule disjI2)
+      apply assumption
+  done
+done
+apply(insert prems1(1,3,5))
+  apply(erule previous_rule)
+  apply simp
+  apply(rule impI)
+  apply(erule impE)
+  apply assumption
+  subgoal premises prems14
+  apply(insert prems14(1,3))
+    apply assumption
+  done
+done
+done
 
 lemma P3_4einv_imp_req_gen: "
 P3_4_inv b_0 b_1 w_0 A11 A12 A2_1 A3_1 s0 \<Longrightarrow>
 toEnvP s0 \<Longrightarrow>
 ((True \<and> True) \<and> ((always_imp s0 (A2_1 s0) (A2 s0)) \<and> (always_imp s0 (A3_1 s0) (A3 s0)))) \<Longrightarrow>
-P3_4 A11 A12 A2 A3 s0"
-  unfolding P3_4_inv_def P3_4_def
-  apply(proveOuter add_rules: inv_req)
-  done
+P3_4 A11 A12 A2 A3 s0"unfolding P3_4_inv_def P3_4_def
+subgoal premises prems1
+apply(insert prems1(1,2))
+apply(simp only: conj_assoc)
+apply(erule conjE)
+subgoal premises prems2
+apply(insert prems2(1,2) prems1(3))
+apply(erule always_einv2req)
+apply simp
+  apply(rule always_disj_rule)
+  apply simp
+    apply(erule conjE)
+    subgoal premises prems3
+    apply(rule conjI)
+    apply(insert prems3(1,2))[1]
+      apply(rule weak_previous_LS5)
+      apply simp
+        apply(rule always_disj_rule)
+        apply simp
+          apply(erule conjE)
+          subgoal premises prems4
+          apply(rule conjI)
+          apply(insert prems4(1,2))[1]
+            apply(rule weak_previous_LS5)
+            apply simp
+              apply(rule always_imp_refl)
+          apply(insert prems4(1,3))
+            apply(rule always_imp_refl)
+          done
+    apply(insert prems3(1,3))
+      apply(rule weak_until_einv2req)
+      apply simp
+        apply(erule conjE)
+        subgoal premises prems5
+        apply(rule conjI)
+        apply(insert prems5(1,2))[1]
+          apply assumption
+        apply(insert prems5(1,3))
+          apply assumption
+        done
+    done
+done
+done
+done
 
 lemma P3_4_inv_saving: "
 P3_4_inv_part b_0 b_1 w_0 A11 A12 A2 A3 s0 \<Longrightarrow>
 consecutive s0 s \<Longrightarrow>
 (((((\<not> (w_0 s0)) \<or> ((A3 s) \<or> ((w_0 s) \<and> (A2 s)))) \<and> ((b_1 s0) \<or> ((A3 s) \<or> ((w_0 s) \<and> (A2 s))))) \<and> ((b_1 s) --> ((b_0 s0) \<or> (\<not> (A12 s))))) \<and> ((b_0 s) --> (\<not> (A11 s)))) \<Longrightarrow>
-P3_4_inv_part b_0 b_1 w_0 A11 A12 A2 A3 s"
-  unfolding P3_4_inv_part_def
-  by(simp add: P3_4_inv_saving_gen always_imp_refl)
+P3_4_inv_part b_0 b_1 w_0 A11 A12 A2 A3 s"unfolding P3_4_inv_part_def P3_4_part_def
+apply(simp add: P3_4_inv_saving_gen always_imp_refl)
+done
 
 lemma P3_4einv_imp_req: "
 P3_4_inv_part b_0 b_1 w_0 A11 A12 A2 A3 s \<Longrightarrow>
 toEnvP s \<Longrightarrow>
 True \<Longrightarrow>
-P3_4_part A11 A12 A2 A3 s"
-  unfolding P3_4_inv_part_def P3_4_part_def
-  by(simp add: P3_4einv_imp_req_gen always_imp_refl)
+P3_4_part A11 A12 A2 A3 s"unfolding P3_4_inv_part_def P3_4_part_def
+apply(simp add: P3_4einv_imp_req_gen always_imp_refl)
+done
 
 lemmas P3_4_used_patterns = P3_4_def always_def weak_previous_def weak_previous_def weak_until_def 
 
@@ -497,8 +1529,6 @@ lemmas P3_4_inv_part_used_patterns = P3_4_inv_part_def P3_4_inv_used_patterns
 
 lemmas P3_4_part_used_patterns = P3_4_part_def P3_4_used_patterns
 
-
-
 definition P4_1 where "P4_1 t A1 A2 A3 s \<equiv> (always (\<lambda> r2 r1 . ((\<not> (A1 r1)) \<or> (constrained_weak_until t A2 A3 r2 r1))) s)"
 
 definition P4_1_part where "P4_1_part t A1 A2 A3 s \<equiv> (P4_1 t A1 (\<lambda> s s1 . (A2 s1)) (\<lambda> s s1 . (A3 s1)) s)"
@@ -507,41 +1537,138 @@ definition P4_1_inv where "P4_1_inv t t1_0 A1 A2_1 A3_1 s \<equiv> (always_inv (
 
 definition P4_1_inv_part where "P4_1_inv_part t t1_0 A1 A2 A3 s \<equiv> (P4_1_inv t t1_0 A1 (\<lambda> s s1 . (A2 s1)) (\<lambda> s s1 . (A3 s1)) s)"
 
-
-
 lemma P4_1_inv_saving_gen: "
 P4_1_inv t t1_0 A1 A2_1 A3_1 s0 \<Longrightarrow>
 consecutive s0 s \<Longrightarrow>
 ((True \<and> ((always_imp s0 (A2_1 s0) (A2_1 s)) \<and> ((always_imp s0 (A3_1 s0) (A3_1 s)) \<and> ((((t1_0 s0) < t) \<and> (((A3_1 s s) \<and> ((t1_0 s) <= (t + 1))) \<or> (((t1_0 s) <= ((t1_0 s0) + 1)) \<and> (A2_1 s s)))) \<or> (((t1_0 s0) >= t) \<and> ((t1_0 s) <= ((t1_0 s0) + 1))))))) \<and> ((\<not> (A1 s)) \<or> ((A3_1 s s) \<or> (((t1_0 s) = 0) \<and> (A2_1 s s))))) \<Longrightarrow>
 P4_1_inv t t1_0 A1 A2_1 A3_1 s"
-  unfolding P4_1_inv_def P4_1_def
-  apply(proveOuter add_rules: invsaving)
+unfolding P4_1_inv_def
+apply(erule always_rule)
+  apply simp
+  apply(erule conjE)
+  subgoal premises prems1
+  apply(rule conjI)
+  apply(insert prems1(1,2))[1]
+    apply(rule always_disj_rule)
+    apply simp
+      apply(erule conjE)
+      subgoal premises prems2
+      apply(rule conjI)
+      apply(insert prems2(1,2))[1]
+        apply(rule always_imp_refl)
+      apply(insert prems2(1,3))
+        apply(rule constrained_weak_until_rule)
+        apply simp
+          apply(erule conjE)
+          subgoal premises prems3
+          apply(rule conjI)
+          apply(insert prems3(1,2))[1]
+            apply assumption
+          apply(insert prems3(1,3))
+            apply(erule conjE)
+            subgoal premises prems4
+            apply(rule conjI)
+            apply(insert prems4(1,2))[1]
+              apply assumption
+            apply(insert prems4(1,3))
+              apply(erule disjE)
+              apply(rule disjI1)
+                apply(erule conjE)
+                subgoal premises prems5
+                apply(rule conjI)
+                apply(insert prems5(1,2))[1]
+                  apply assumption
+                apply(insert prems5(1,3))
+                  apply(erule disjE)
+                  apply(rule disjI1)
+                    apply(erule conjE)
+                    subgoal premises prems6
+                    apply(rule conjI)
+                    apply(insert prems6(1,2))[1]
+                      apply assumption
+                    apply(insert prems6(1,3))
+                      apply assumption
+                    done
+                  apply(rule disjI2)
+                    apply(erule conjE)
+                    subgoal premises prems7
+                    apply(rule conjI)
+                    apply(insert prems7(1,2))[1]
+                      apply assumption
+                    apply(insert prems7(1,3))
+                      apply assumption
+                    done
+                done
+              apply(rule disjI2)
+                apply assumption
+            done
+          done
+      done
+  apply(insert prems1(1,3))
+    apply(erule disjE)
+    apply(rule disjI1)
+      apply assumption
+    apply(rule disjI2)
+      apply(rule constrained_weak_until_one_point)
+      apply simp
+        apply(erule disjE)
+        apply(rule disjI1)
+          apply assumption
+        apply(rule disjI2)
+          apply(erule conjE)
+          subgoal premises prems8
+          apply(rule conjI)
+          apply(insert prems8(1,2))[1]
+            apply assumption
+          apply(insert prems8(1,3))
+            apply assumption
+          done
   done
+done
 
 lemma P4_1einv_imp_req_gen: "
 P4_1_inv t t1_0 A1 A2_1 A3_1 s0 \<Longrightarrow>
 toEnvP s0 \<Longrightarrow>
 (True \<and> ((always_imp s0 (A2_1 s0) (A2 s0)) \<and> (always_imp s0 (A3_1 s0) (A3 s0)))) \<Longrightarrow>
-P4_1 t A1 A2 A3 s0"
-  unfolding P4_1_inv_def P4_1_def
-  apply(proveOuter add_rules: inv_req)
-  done
+P4_1 t A1 A2 A3 s0"unfolding P4_1_inv_def P4_1_def
+apply(erule always_einv2req)
+apply simp
+  apply(rule always_disj_rule)
+  apply simp
+    apply(erule conjE)
+    subgoal premises prems3
+    apply(rule conjI)
+    apply(insert prems3(1,2))[1]
+      apply(rule always_imp_refl)
+    apply(insert prems3(1,3))
+      apply(rule constrained_weak_until_einv2req)
+      apply simp
+        apply(erule conjE)
+        subgoal premises prems4
+        apply(rule conjI)
+        apply(insert prems4(1,2))[1]
+          apply assumption
+        apply(insert prems4(1,3))
+          apply assumption
+        done
+    done
+done
 
 lemma P4_1_inv_saving: "
 P4_1_inv_part t t1_0 A1 A2 A3 s0 \<Longrightarrow>
 consecutive s0 s \<Longrightarrow>
 (((((t1_0 s0) < t) \<and> (((A3 s) \<and> ((t1_0 s) <= (t + 1))) \<or> (((t1_0 s) <= ((t1_0 s0) + 1)) \<and> (A2 s)))) \<or> (((t1_0 s0) >= t) \<and> ((t1_0 s) <= ((t1_0 s0) + 1)))) \<and> ((\<not> (A1 s)) \<or> ((A3 s) \<or> (((t1_0 s) = 0) \<and> (A2 s))))) \<Longrightarrow>
-P4_1_inv_part t t1_0 A1 A2 A3 s"
-  unfolding P4_1_inv_part_def
-  by(simp add: P4_1_inv_saving_gen always_imp_refl)
+P4_1_inv_part t t1_0 A1 A2 A3 s"unfolding P4_1_inv_part_def P4_1_part_def
+apply(simp add: P4_1_inv_saving_gen always_imp_refl)
+done
 
 lemma P4_1einv_imp_req: "
 P4_1_inv_part t t1_0 A1 A2 A3 s \<Longrightarrow>
 toEnvP s \<Longrightarrow>
 True \<Longrightarrow>
-P4_1_part t A1 A2 A3 s"
-  unfolding P4_1_inv_part_def P4_1_part_def
-  by(simp add: P4_1einv_imp_req_gen always_imp_refl)
+P4_1_part t A1 A2 A3 s"unfolding P4_1_inv_part_def P4_1_part_def
+apply(simp add: P4_1einv_imp_req_gen always_imp_refl)
+done
 
 lemmas P4_1_used_patterns = P4_1_def always_def constrained_weak_until_def 
 
@@ -551,52 +1678,204 @@ lemmas P4_1_inv_part_used_patterns = P4_1_inv_part_def P4_1_inv_used_patterns
 
 lemmas P4_1_part_used_patterns = P4_1_part_def P4_1_used_patterns
 
-
-
-
 definition P4_2 where "P4_2 t A11 A12 A2 A3 s \<equiv> (always (\<lambda> r2 r1 . ((weak_previous (\<lambda> r4 r3 . (\<not> (A11 r3))) r2 r1) \<or> ((\<not> (A12 r1)) \<or> (constrained_weak_until t A2 A3 r2 r1)))) s)"
 
 definition P4_2_part where "P4_2_part t A11 A12 A2 A3 s \<equiv> (P4_2 t A11 A12 (\<lambda> s s1 . (A2 s1)) (\<lambda> s s1 . (A3 s1)) s)"
 
-definition P4_2_inv where "P4_2_inv t b_0 t1_0 A11 A12 A2_1 A3_1 s \<equiv> ((always_inv (\<lambda> r2 r1 . ((weak_previous (\<lambda> r4 r3 . (\<not> (A11 r3))) r2 r1) \<or> ((\<not> (A12 r1)) \<or> (constrained_weak_until_inv t t1_0 A2_1 A3_1 r2 r1)))) s) \<and> (b_0 s --> (previous_inv (\<lambda> r4 r3 . (\<not> (A11 r3))) s)))"
+definition P4_2_inv where "P4_2_inv t b_0 t1_0 A11 A12 A2_1 A3_1 s \<equiv> ((always_inv (\<lambda> r2 r1 . ((weak_previous (\<lambda> r4 r3 . (\<not> (A11 r3))) r2 r1) \<or> ((\<not> (A12 r1)) \<or> (constrained_weak_until_inv t t1_0 A2_1 A3_1 r2 r1)))) s) \<and> (previous_inv b_0 (\<lambda> r4 r3 . (\<not> (A11 r3))) s))"
 
 definition P4_2_inv_part where "P4_2_inv_part t b_0 t1_0 A11 A12 A2 A3 s \<equiv> (P4_2_inv t b_0 t1_0 A11 A12 (\<lambda> s s1 . (A2 s1)) (\<lambda> s s1 . (A3 s1)) s)"
-
-
 
 lemma P4_2_inv_saving_gen: "
 P4_2_inv t b_0 t1_0 A11 A12 A2_1 A3_1 s0 \<Longrightarrow>
 consecutive s0 s \<Longrightarrow>
 (((True \<and> (True \<and> ((always_imp s0 (A2_1 s0) (A2_1 s)) \<and> ((always_imp s0 (A3_1 s0) (A3_1 s)) \<and> ((((t1_0 s0) < t) \<and> (((A3_1 s s) \<and> ((t1_0 s) <= (t + 1))) \<or> (((t1_0 s) <= ((t1_0 s0) + 1)) \<and> (A2_1 s s)))) \<or> (((t1_0 s0) >= t) \<and> ((t1_0 s) <= ((t1_0 s0) + 1)))))))) \<and> (((b_0 s0) \<and> True) \<or> ((\<not> (A12 s)) \<or> ((A3_1 s s) \<or> (((t1_0 s) = 0) \<and> (A2_1 s s)))))) \<and> ((b_0 s) --> (\<not> (A11 s)))) \<Longrightarrow>
 P4_2_inv t b_0 t1_0 A11 A12 A2_1 A3_1 s"
-  unfolding P4_2_inv_def P4_2_def
-  apply(proveOuter add_rules: invsaving)
+unfolding P4_2_inv_def
+apply(erule conjE)
+apply(erule conjE)
+subgoal premises prems1
+apply(rule conjI)
+apply(insert prems1(1,2,4))[1]
+apply(erule always_rule)
+  apply simp
+  apply(erule conjE)
+  subgoal premises prems2
+  apply(rule conjI)
+  apply(insert prems2(1,2))[1]
+    apply(rule always_disj_rule)
+    apply simp
+      apply(erule conjE)
+      subgoal premises prems3
+      apply(rule conjI)
+      apply(insert prems3(1,2))[1]
+        apply(rule weak_previous_LS4)
+        apply simp
+          apply(rule always_imp_refl)
+      apply(insert prems3(1,3))
+        apply(rule always_disj_rule)
+        apply simp
+          apply(erule conjE)
+          subgoal premises prems4
+          apply(rule conjI)
+          apply(insert prems4(1,2))[1]
+            apply(rule always_imp_refl)
+          apply(insert prems4(1,3))
+            apply(rule constrained_weak_until_rule)
+            apply simp
+              apply(erule conjE)
+              subgoal premises prems5
+              apply(rule conjI)
+              apply(insert prems5(1,2))[1]
+                apply assumption
+              apply(insert prems5(1,3))
+                apply(erule conjE)
+                subgoal premises prems6
+                apply(rule conjI)
+                apply(insert prems6(1,2))[1]
+                  apply assumption
+                apply(insert prems6(1,3))
+                  apply(erule disjE)
+                  apply(rule disjI1)
+                    apply(erule conjE)
+                    subgoal premises prems7
+                    apply(rule conjI)
+                    apply(insert prems7(1,2))[1]
+                      apply assumption
+                    apply(insert prems7(1,3))
+                      apply(erule disjE)
+                      apply(rule disjI1)
+                        apply(erule conjE)
+                        subgoal premises prems8
+                        apply(rule conjI)
+                        apply(insert prems8(1,2))[1]
+                          apply assumption
+                        apply(insert prems8(1,3))
+                          apply assumption
+                        done
+                      apply(rule disjI2)
+                        apply(erule conjE)
+                        subgoal premises prems9
+                        apply(rule conjI)
+                        apply(insert prems9(1,2))[1]
+                          apply assumption
+                        apply(insert prems9(1,3))
+                          apply assumption
+                        done
+                    done
+                  apply(rule disjI2)
+                    apply assumption
+                done
+              done
+          done
+      done
+  apply(insert prems2(1,3))
+    apply(erule disjE)
+    apply(rule disjI1)
+      apply(rule weak_previous_one_point[OF prems1(3)])
+      apply simp
+        apply(erule conjE)
+        subgoal premises prems10
+        apply(rule conjI)
+        apply(insert prems10(1,2))[1]
+          apply assumption
+        apply(insert prems10(1,3))
+          apply(rule always_imp_refl)
+        done
+    apply(rule disjI2)
+      apply(erule disjE)
+      apply(rule disjI1)
+        apply assumption
+      apply(rule disjI2)
+        apply(rule constrained_weak_until_one_point)
+        apply simp
+          apply(erule disjE)
+          apply(rule disjI1)
+            apply assumption
+          apply(rule disjI2)
+            apply(erule conjE)
+            subgoal premises prems11
+            apply(rule conjI)
+            apply(insert prems11(1,2))[1]
+              apply assumption
+            apply(insert prems11(1,3))
+              apply assumption
+            done
   done
+apply(insert prems1(1,3,5))
+  apply(erule previous_rule)
+  apply simp
+  apply(rule impI)
+  apply(erule impE)
+  apply assumption
+  subgoal premises prems12
+  apply(insert prems12(1,3))
+    apply assumption
+  done
+done
+done
 
 lemma P4_2einv_imp_req_gen: "
 P4_2_inv t b_0 t1_0 A11 A12 A2_1 A3_1 s0 \<Longrightarrow>
 toEnvP s0 \<Longrightarrow>
 (True \<and> (True \<and> ((always_imp s0 (A2_1 s0) (A2 s0)) \<and> (always_imp s0 (A3_1 s0) (A3 s0))))) \<Longrightarrow>
-P4_2 t A11 A12 A2 A3 s0"
-  unfolding P4_2_inv_def P4_2_def
-  apply(proveOuter add_rules: inv_req)
-  done
+P4_2 t A11 A12 A2 A3 s0"unfolding P4_2_inv_def P4_2_def
+subgoal premises prems1
+apply(insert prems1(1,2))
+apply(erule conjE)
+subgoal premises prems2
+apply(insert prems2(1,2) prems1(3))
+apply(erule always_einv2req)
+apply simp
+  apply(rule always_disj_rule)
+  apply simp
+    apply(erule conjE)
+    subgoal premises prems3
+    apply(rule conjI)
+    apply(insert prems3(1,2))[1]
+      apply(rule weak_previous_LS5)
+      apply simp
+        apply(rule always_imp_refl)
+    apply(insert prems3(1,3))
+      apply(rule always_disj_rule)
+      apply simp
+        apply(erule conjE)
+        subgoal premises prems4
+        apply(rule conjI)
+        apply(insert prems4(1,2))[1]
+          apply(rule always_imp_refl)
+        apply(insert prems4(1,3))
+          apply(rule constrained_weak_until_einv2req)
+          apply simp
+            apply(erule conjE)
+            subgoal premises prems5
+            apply(rule conjI)
+            apply(insert prems5(1,2))[1]
+              apply assumption
+            apply(insert prems5(1,3))
+              apply assumption
+            done
+        done
+    done
+done
+done
+done
 
 lemma P4_2_inv_saving: "
 P4_2_inv_part t b_0 t1_0 A11 A12 A2 A3 s0 \<Longrightarrow>
 consecutive s0 s \<Longrightarrow>
 ((((((t1_0 s0) < t) \<and> (((A3 s) \<and> ((t1_0 s) <= (t + 1))) \<or> (((t1_0 s) <= ((t1_0 s0) + 1)) \<and> (A2 s)))) \<or> (((t1_0 s0) >= t) \<and> ((t1_0 s) <= ((t1_0 s0) + 1)))) \<and> ((b_0 s0) \<or> ((\<not> (A12 s)) \<or> ((A3 s) \<or> (((t1_0 s) = 0) \<and> (A2 s)))))) \<and> ((b_0 s) --> (\<not> (A11 s)))) \<Longrightarrow>
-P4_2_inv_part t b_0 t1_0 A11 A12 A2 A3 s"
-  unfolding P4_2_inv_part_def
-  by(simp add: P4_2_inv_saving_gen always_imp_refl)
+P4_2_inv_part t b_0 t1_0 A11 A12 A2 A3 s"unfolding P4_2_inv_part_def P4_2_part_def
+apply(simp add: P4_2_inv_saving_gen always_imp_refl)
+done
 
 lemma P4_2einv_imp_req: "
 P4_2_inv_part t b_0 t1_0 A11 A12 A2 A3 s \<Longrightarrow>
 toEnvP s \<Longrightarrow>
 True \<Longrightarrow>
-P4_2_part t A11 A12 A2 A3 s"
-  unfolding P4_2_inv_part_def P4_2_part_def
-  by(simp add: P4_2einv_imp_req_gen always_imp_refl)
+P4_2_part t A11 A12 A2 A3 s"unfolding P4_2_inv_part_def P4_2_part_def
+apply(simp add: P4_2einv_imp_req_gen always_imp_refl)
+done
 
 lemmas P4_2_used_patterns = P4_2_def always_def weak_previous_def constrained_weak_until_def 
 
@@ -606,54 +1885,275 @@ lemmas P4_2_inv_part_used_patterns = P4_2_inv_part_def P4_2_inv_used_patterns
 
 lemmas P4_2_part_used_patterns = P4_2_part_def P4_2_used_patterns
 
-
-
-
 definition P4_3 where "P4_3 t A11 A12 A21 A22 A3 s \<equiv> (always (\<lambda> r2 r1 . ((weak_previous (\<lambda> r4 r3 . (\<not> (A11 r3))) r2 r1) \<or> ((\<not> (A12 r1)) \<or> (constrained_weak_until t (\<lambda> r4 r3 . ((previous A21 r4 r3) \<and> (A22 r4 r3))) A3 r2 r1)))) s)"
 
 definition P4_3_part where "P4_3_part t A11 A12 A21 A22 A3 s \<equiv> (P4_3 t A11 A12 (\<lambda> s s1 . (A21 s1)) (\<lambda> s s1 . (A22 s1)) (\<lambda> s s1 . (A3 s1)) s)"
 
-definition P4_3_inv where "P4_3_inv t b_0 b_1 t1_0 A11 A12 A21_1 A22_1 A3_1 s \<equiv> (((always_inv (\<lambda> r2 r1 . ((weak_previous (\<lambda> r4 r3 . (\<not> (A11 r3))) r2 r1) \<or> ((\<not> (A12 r1)) \<or> (constrained_weak_until_inv t t1_0 (\<lambda> r4 r3 . ((previous A21_1 r4 r3) \<and> (A22_1 r4 r3))) A3_1 r2 r1)))) s) \<and> (b_0 s --> (previous_inv (\<lambda> r4 r3 . (\<not> (A11 r3))) s))) \<and> (b_1 s --> (previous_inv A21_1 s)))"
+definition P4_3_inv where "P4_3_inv t b_0 b_1 t1_0 A11 A12 A21_1 A22_1 A3_1 s \<equiv> (((always_inv (\<lambda> r2 r1 . ((weak_previous (\<lambda> r4 r3 . (\<not> (A11 r3))) r2 r1) \<or> ((\<not> (A12 r1)) \<or> (constrained_weak_until_inv t t1_0 (\<lambda> r4 r3 . ((previous A21_1 r4 r3) \<and> (A22_1 r4 r3))) A3_1 r2 r1)))) s) \<and> (previous_inv b_0 (\<lambda> r4 r3 . (\<not> (A11 r3))) s)) \<and> (previous_inv b_1 A21_1 s))"
 
 definition P4_3_inv_part where "P4_3_inv_part t b_0 b_1 t1_0 A11 A12 A21 A22 A3 s \<equiv> (P4_3_inv t b_0 b_1 t1_0 A11 A12 (\<lambda> s s1 . (A21 s1)) (\<lambda> s s1 . (A22 s1)) (\<lambda> s s1 . (A3 s1)) s)"
-
-
 
 lemma P4_3_inv_saving_gen: "
 P4_3_inv t b_0 b_1 t1_0 A11 A12 A21_1 A22_1 A3_1 s0 \<Longrightarrow>
 consecutive s0 s \<Longrightarrow>
 ((((True \<and> (True \<and> (((always_imp s0 (A21_1 s0) (A21_1 s)) \<and> (always_imp s0 (\<lambda> r3 . (A22_1 s0 r3)) (\<lambda> r3 . (A22_1 s r3)))) \<and> ((always_imp s0 (A3_1 s0) (A3_1 s)) \<and> ((((t1_0 s0) < t) \<and> (((A3_1 s s) \<and> ((t1_0 s) <= (t + 1))) \<or> (((t1_0 s) <= ((t1_0 s0) + 1)) \<and> (((b_1 s0) \<and> (always_imp s0 (A21_1 s0) (A21_1 s))) \<and> (A22_1 s s))))) \<or> (((t1_0 s0) >= t) \<and> ((t1_0 s) <= ((t1_0 s0) + 1)))))))) \<and> (((b_0 s0) \<and> True) \<or> ((\<not> (A12 s)) \<or> ((A3_1 s s) \<or> (((t1_0 s) = 0) \<and> (((b_1 s0) \<and> (always_imp s0 (A21_1 s0) (A21_1 s))) \<and> (A22_1 s s))))))) \<and> ((b_0 s) --> (\<not> (A11 s)))) \<and> ((b_1 s) --> (A21_1 s s))) \<Longrightarrow>
 P4_3_inv t b_0 b_1 t1_0 A11 A12 A21_1 A22_1 A3_1 s"
-  unfolding P4_3_inv_def P4_3_def
-  apply(proveOuter add_rules: invsaving)
+unfolding P4_3_inv_def
+apply(erule conjE)
+apply(erule conjE)
+subgoal premises prems1
+apply(rule conjI)
+apply(insert prems1(1,2,4))[1]
+apply(erule conjE)
+apply(erule conjE)
+subgoal premises prems2
+apply(rule conjI)
+apply(insert prems2(1,2,4))[1]
+apply(erule always_rule)
+  apply simp
+  apply(erule conjE)
+  subgoal premises prems3
+  apply(rule conjI)
+  apply(insert prems3(1,2))[1]
+    apply(rule always_disj_rule)
+    apply simp
+      apply(erule conjE)
+      subgoal premises prems4
+      apply(rule conjI)
+      apply(insert prems4(1,2))[1]
+        apply(rule weak_previous_LS4)
+        apply simp
+          apply(rule always_imp_refl)
+      apply(insert prems4(1,3))
+        apply(rule always_disj_rule)
+        apply simp
+          apply(erule conjE)
+          subgoal premises prems5
+          apply(rule conjI)
+          apply(insert prems5(1,2))[1]
+            apply(rule always_imp_refl)
+          apply(insert prems5(1,3))
+            apply(rule constrained_weak_until_rule)
+            apply simp
+              apply(erule conjE)
+              subgoal premises prems6
+              apply(rule conjI)
+              apply(insert prems6(1,2))[1]
+                apply(rule always_conj_rule)
+                apply simp
+                  apply(erule conjE)
+                  subgoal premises prems7
+                  apply(rule conjI)
+                  apply(insert prems7(1,2))[1]
+                    apply(rule previous_LS4)
+                    apply simp
+                      apply assumption
+                  apply(insert prems7(1,3))
+                    apply assumption
+                  done
+              apply(insert prems6(1,3))
+                apply(erule conjE)
+                subgoal premises prems8
+                apply(rule conjI)
+                apply(insert prems8(1,2))[1]
+                  apply assumption
+                apply(insert prems8(1,3))
+                  apply(erule disjE)
+                  apply(rule disjI1)
+                    apply(erule conjE)
+                    subgoal premises prems9
+                    apply(rule conjI)
+                    apply(insert prems9(1,2))[1]
+                      apply assumption
+                    apply(insert prems9(1,3))
+                      apply(erule disjE)
+                      apply(rule disjI1)
+                        apply(erule conjE)
+                        subgoal premises prems10
+                        apply(rule conjI)
+                        apply(insert prems10(1,2))[1]
+                          apply assumption
+                        apply(insert prems10(1,3))
+                          apply assumption
+                        done
+                      apply(rule disjI2)
+                        apply(erule conjE)
+                        subgoal premises prems11
+                        apply(rule conjI)
+                        apply(insert prems11(1,2))[1]
+                          apply assumption
+                        apply(insert prems11(1,3))
+                          apply(erule conjE)
+                          subgoal premises prems12
+                          apply(rule conjI)
+                          apply(insert prems12(1,2))[1]
+                            apply(rule previous_one_point[OF prems1(3)])
+                            apply simp
+                              apply(erule conjE)
+                              subgoal premises prems13
+                              apply(rule conjI)
+                              apply(insert prems13(1,2))[1]
+                                apply assumption
+                              apply(insert prems13(1,3))
+                                apply assumption
+                              done
+                          apply(insert prems12(1,3))
+                            apply assumption
+                          done
+                        done
+                    done
+                  apply(rule disjI2)
+                    apply assumption
+                done
+              done
+          done
+      done
+  apply(insert prems3(1,3))
+    apply(erule disjE)
+    apply(rule disjI1)
+      apply(rule weak_previous_one_point[OF prems2(3)])
+      apply simp
+        apply(erule conjE)
+        subgoal premises prems14
+        apply(rule conjI)
+        apply(insert prems14(1,2))[1]
+          apply assumption
+        apply(insert prems14(1,3))
+          apply(rule always_imp_refl)
+        done
+    apply(rule disjI2)
+      apply(erule disjE)
+      apply(rule disjI1)
+        apply assumption
+      apply(rule disjI2)
+        apply(rule constrained_weak_until_one_point)
+        apply simp
+          apply(erule disjE)
+          apply(rule disjI1)
+            apply assumption
+          apply(rule disjI2)
+            apply(erule conjE)
+            subgoal premises prems15
+            apply(rule conjI)
+            apply(insert prems15(1,2))[1]
+              apply assumption
+            apply(insert prems15(1,3))
+              apply(erule conjE)
+              subgoal premises prems16
+              apply(rule conjI)
+              apply(insert prems16(1,2))[1]
+                apply(rule previous_one_point[OF prems1(3)])
+                apply simp
+                  apply(erule conjE)
+                  subgoal premises prems17
+                  apply(rule conjI)
+                  apply(insert prems17(1,2))[1]
+                    apply assumption
+                  apply(insert prems17(1,3))
+                    apply assumption
+                  done
+              apply(insert prems16(1,3))
+                apply assumption
+              done
+            done
   done
+apply(insert prems2(1,3,5))
+  apply(erule previous_rule)
+  apply simp
+  apply(rule impI)
+  apply(erule impE)
+  apply assumption
+  subgoal premises prems18
+  apply(insert prems18(1,3))
+    apply assumption
+  done
+done
+apply(insert prems1(1,3,5))
+  apply(erule previous_rule)
+  apply simp
+  apply(rule impI)
+  apply(erule impE)
+  apply assumption
+  subgoal premises prems19
+  apply(insert prems19(1,3))
+    apply assumption
+  done
+done
+done
 
 lemma P4_3einv_imp_req_gen: "
 P4_3_inv t b_0 b_1 t1_0 A11 A12 A21_1 A22_1 A3_1 s0 \<Longrightarrow>
 toEnvP s0 \<Longrightarrow>
 (True \<and> (True \<and> (((always_imp s0 (A21_1 s0) (A21 s0)) \<and> (always_imp s0 (\<lambda> r3 . (A22_1 s0 r3)) (\<lambda> r3 . (A22 s0 r3)))) \<and> (always_imp s0 (A3_1 s0) (A3 s0))))) \<Longrightarrow>
-P4_3 t A11 A12 A21 A22 A3 s0"
-  unfolding P4_3_inv_def P4_3_def
-  apply(proveOuter add_rules: inv_req)
-  done
+P4_3 t A11 A12 A21 A22 A3 s0"unfolding P4_3_inv_def P4_3_def
+subgoal premises prems1
+apply(insert prems1(1,2))
+apply(simp only: conj_assoc)
+apply(erule conjE)
+subgoal premises prems2
+apply(insert prems2(1,2) prems1(3))
+apply(erule always_einv2req)
+apply simp
+  apply(rule always_disj_rule)
+  apply simp
+    apply(erule conjE)
+    subgoal premises prems3
+    apply(rule conjI)
+    apply(insert prems3(1,2))[1]
+      apply(rule weak_previous_LS5)
+      apply simp
+        apply(rule always_imp_refl)
+    apply(insert prems3(1,3))
+      apply(rule always_disj_rule)
+      apply simp
+        apply(erule conjE)
+        subgoal premises prems4
+        apply(rule conjI)
+        apply(insert prems4(1,2))[1]
+          apply(rule always_imp_refl)
+        apply(insert prems4(1,3))
+          apply(rule constrained_weak_until_einv2req)
+          apply simp
+            apply(erule conjE)
+            subgoal premises prems5
+            apply(rule conjI)
+            apply(insert prems5(1,2))[1]
+              apply(rule always_conj_rule)
+              apply simp
+                apply(erule conjE)
+                subgoal premises prems6
+                apply(rule conjI)
+                apply(insert prems6(1,2))[1]
+                  apply(rule previous_LS5)
+                  apply simp
+                    apply assumption
+                apply(insert prems6(1,3))
+                  apply assumption
+                done
+            apply(insert prems5(1,3))
+              apply assumption
+            done
+        done
+    done
+done
+done
+done
 
 lemma P4_3_inv_saving: "
 P4_3_inv_part t b_0 b_1 t1_0 A11 A12 A21 A22 A3 s0 \<Longrightarrow>
 consecutive s0 s \<Longrightarrow>
 (((((((t1_0 s0) < t) \<and> (((A3 s) \<and> ((t1_0 s) <= (t + 1))) \<or> (((t1_0 s) <= ((t1_0 s0) + 1)) \<and> ((b_1 s0) \<and> (A22 s))))) \<or> (((t1_0 s0) >= t) \<and> ((t1_0 s) <= ((t1_0 s0) + 1)))) \<and> ((b_0 s0) \<or> ((\<not> (A12 s)) \<or> ((A3 s) \<or> (((t1_0 s) = 0) \<and> ((b_1 s0) \<and> (A22 s))))))) \<and> ((b_0 s) --> (\<not> (A11 s)))) \<and> ((b_1 s) --> (A21 s))) \<Longrightarrow>
-P4_3_inv_part t b_0 b_1 t1_0 A11 A12 A21 A22 A3 s"
-  unfolding P4_3_inv_part_def
-  apply(simp add: P4_3_inv_saving_gen always_imp_refl)
-  done
+P4_3_inv_part t b_0 b_1 t1_0 A11 A12 A21 A22 A3 s"unfolding P4_3_inv_part_def P4_3_part_def
+apply(simp add: P4_3_inv_saving_gen always_imp_refl)
+done
 
 lemma P4_3einv_imp_req: "
 P4_3_inv_part t b_0 b_1 t1_0 A11 A12 A21 A22 A3 s \<Longrightarrow>
 toEnvP s \<Longrightarrow>
 True \<Longrightarrow>
-P4_3_part t A11 A12 A21 A22 A3 s"
-  unfolding P4_3_inv_part_def P4_3_part_def
-  apply(simp add: P4_3einv_imp_req_gen always_imp_refl)
-  done
+P4_3_part t A11 A12 A21 A22 A3 s"unfolding P4_3_inv_part_def P4_3_part_def
+apply(simp add: P4_3einv_imp_req_gen always_imp_refl)
+done
 
 lemmas P4_3_used_patterns = P4_3_def always_def weak_previous_def constrained_weak_until_def previous_def 
 
@@ -663,5 +2163,561 @@ lemmas P4_3_inv_part_used_patterns = P4_3_inv_part_def P4_3_inv_used_patterns
 
 lemmas P4_3_part_used_patterns = P4_3_part_def P4_3_used_patterns
 
+definition P6_1 where "P6_1 t A1 A2 A3 A4 s \<equiv> (always (\<lambda> r2 r1 . ((weak_previous (\<lambda> r4 r3 . (dual_since t (\<lambda> r6 r5 . (\<not> (A2 r5))) (\<lambda> r6 r5 . (\<not> (A1 r5))) r4 r3)) r2 r1) \<or> ((\<not> (A3 r1)) \<or> (A4 r2 r1)))) s)"
+
+definition P6_1_part where "P6_1_part t A1 A2 A3 A4 s \<equiv> (P6_1 t A1 A2 A3 (\<lambda> s s1 . (A4 s1)) s)"
+
+definition P6_1_inv where "P6_1_inv t b_0 t1_0 b_1 A1 A2 A3 A4_1 s \<equiv> (((always_inv (\<lambda> r2 r1 . ((weak_previous (\<lambda> r4 r3 . (dual_since t (\<lambda> r6 r5 . (\<not> (A2 r5))) (\<lambda> r6 r5 . (\<not> (A1 r5))) r4 r3)) r2 r1) \<or> ((\<not> (A3 r1)) \<or> (A4_1 r2 r1)))) s) \<and> (previous_inv b_1 (\<lambda> r4 r3 . (dual_since t (\<lambda> r6 r5 . (\<not> (A2 r5))) (\<lambda> r6 r5 . (\<not> (A1 r5))) r4 r3)) s)) \<and> (dual_since_inv t b_0 t1_0 (\<lambda> r6 r5 . (\<not> (A2 r5))) (\<lambda> r6 r5 . (\<not> (A1 r5))) s))"
+
+definition P6_1_inv_part where "P6_1_inv_part t b_0 t1_0 b_1 A1 A2 A3 A4 s \<equiv> (P6_1_inv t b_0 t1_0 b_1 A1 A2 A3 (\<lambda> s s1 . (A4 s1)) s)"
+
+lemma P6_1_inv_saving_gen: "
+P6_1_inv t b_0 t1_0 b_1 A1 A2 A3 A4_1 s0 \<Longrightarrow>
+consecutive s0 s \<Longrightarrow>
+(((((True \<and> True) \<and> (True \<and> (always_imp s0 (\<lambda> r1 . (A4_1 s0 r1)) (\<lambda> r1 . (A4_1 s r1))))) \<and> (((b_1 s0) \<and> (True \<and> True)) \<or> ((\<not> (A3 s)) \<or> (A4_1 s s)))) \<and> ((b_1 s) --> (((t > 0) \<or> (\<not> (A1 s))) \<and> ((\<not> (A2 s)) \<or> ((b_0 s0) \<and> (True \<and> (True \<and> ((t1_0 s0) < t)))))))) \<and> ((((t1_0 s) > 0) \<or> (\<not> (A1 s))) \<and> ((\<not> (A2 s)) \<or> ((b_0 s0) \<and> (True \<and> (True \<and> ((t1_0 s0) < (t1_0 s)))))))) \<Longrightarrow>
+P6_1_inv t b_0 t1_0 b_1 A1 A2 A3 A4_1 s"
+unfolding P6_1_inv_def
+apply(erule conjE)
+apply(erule conjE)
+subgoal premises prems1
+apply(rule conjI)
+apply(insert prems1(1,2,4))[1]
+apply(erule conjE)
+apply(erule conjE)
+subgoal premises prems2
+apply(rule conjI)
+apply(insert prems2(1,2,4))[1]
+apply(erule always_rule)
+  apply simp
+  apply(erule conjE)
+  subgoal premises prems3
+  apply(rule conjI)
+  apply(insert prems3(1,2))[1]
+    apply(rule always_disj_rule)
+    apply simp
+      apply(erule conjE)
+      subgoal premises prems4
+      apply(rule conjI)
+      apply(insert prems4(1,2))[1]
+        apply(rule weak_previous_LS4)
+        apply simp
+          apply(rule dual_since_L4)
+          apply simp
+            apply(erule conjE)
+            subgoal premises prems5
+            apply(rule conjI)
+            apply(insert prems5(1,2))[1]
+              apply(rule always_imp_refl)
+            apply(insert prems5(1,3))
+              apply(rule always_imp_refl)
+            done
+      apply(insert prems4(1,3))
+        apply(rule always_disj_rule)
+        apply simp
+          apply(erule conjE)
+          subgoal premises prems6
+          apply(rule conjI)
+          apply(insert prems6(1,2))[1]
+            apply(rule always_imp_refl)
+          apply(insert prems6(1,3))
+            apply assumption
+          done
+      done
+  apply(insert prems3(1,3))
+    apply(erule disjE)
+    apply(rule disjI1)
+      apply(rule weak_previous_one_point[OF prems2(3)])
+      apply simp
+        apply(erule conjE)
+        subgoal premises prems7
+        apply(rule conjI)
+        apply(insert prems7(1,2))[1]
+          apply assumption
+        apply(insert prems7(1,3))
+          apply(rule dual_since_L4)
+          apply simp
+            apply(erule conjE)
+            subgoal premises prems8
+            apply(rule conjI)
+            apply(insert prems8(1,2))[1]
+              apply(rule always_imp_refl)
+            apply(insert prems8(1,3))
+              apply(rule always_imp_refl)
+            done
+        done
+    apply(rule disjI2)
+      apply(erule disjE)
+      apply(rule disjI1)
+        apply assumption
+      apply(rule disjI2)
+        apply assumption
+  done
+apply(insert prems2(1,3,5))
+  apply(erule previous_rule)
+  apply simp
+  apply(rule impI)
+  apply(erule impE)
+  apply assumption
+  subgoal premises prems9
+  apply(insert prems9(1,3))
+    apply(rule dual_since_L7[OF prems1(3)])
+    apply simp
+      apply(erule conjE)
+      subgoal premises prems10
+      apply(rule conjI)
+      apply(insert prems10(1,2))[1]
+        apply(erule disjE)
+        apply(rule disjI1)
+          apply assumption
+        apply(rule disjI2)
+          apply assumption
+      apply(insert prems10(1,3))
+        apply(erule disjE)
+        apply(rule disjI1)
+          apply assumption
+        apply(rule disjI2)
+          apply(erule conjE)
+          subgoal premises prems11
+          apply(rule conjI)
+          apply(insert prems11(1,2))[1]
+            apply assumption
+          apply(insert prems11(1,3))
+            apply(erule conjE)
+            subgoal premises prems12
+            apply(rule conjI)
+            apply(insert prems12(1,2))[1]
+              apply(rule always_imp_refl)
+            apply(insert prems12(1,3))
+              apply(erule conjE)
+              subgoal premises prems13
+              apply(rule conjI)
+              apply(insert prems13(1,2))[1]
+                apply(rule always_imp_refl)
+              apply(insert prems13(1,3))
+                apply assumption
+              done
+            done
+          done
+      done
+  done
+done
+apply(insert prems1(1,3,5))
+  apply(erule dual_since_one_point)
+  apply simp
+  apply(erule conjE)
+  subgoal premises prems14
+  apply(rule conjI)
+  apply(insert prems14(1,2))[1]
+    apply(erule disjE)
+    apply(rule disjI1)
+      apply assumption
+    apply(rule disjI2)
+      apply assumption
+  apply(insert prems14(1,3))
+    apply(erule disjE)
+    apply(rule disjI1)
+      apply assumption
+    apply(rule disjI2)
+      apply(erule conjE)
+      subgoal premises prems15
+      apply(rule conjI)
+      apply(insert prems15(1,2))[1]
+        apply assumption
+      apply(insert prems15(1,3))
+        apply(erule conjE)
+        subgoal premises prems16
+        apply(rule conjI)
+        apply(insert prems16(1,2))[1]
+          apply(rule always_imp_refl)
+        apply(insert prems16(1,3))
+          apply(erule conjE)
+          subgoal premises prems17
+          apply(rule conjI)
+          apply(insert prems17(1,2))[1]
+            apply(rule always_imp_refl)
+          apply(insert prems17(1,3))
+            apply assumption
+          done
+        done
+      done
+  done
+done
+done
+
+lemma P6_1einv_imp_req_gen: "
+P6_1_inv t b_0 t1_0 b_1 A1 A2 A3 A4_1 s0 \<Longrightarrow>
+toEnvP s0 \<Longrightarrow>
+((True \<and> True) \<and> (True \<and> (always_imp s0 (\<lambda> r1 . (A4_1 s0 r1)) (\<lambda> r1 . (A4 s0 r1))))) \<Longrightarrow>
+P6_1 t A1 A2 A3 A4 s0"unfolding P6_1_inv_def P6_1_def
+subgoal premises prems1
+apply(insert prems1(1,2))
+apply(simp only: conj_assoc)
+apply(erule conjE)
+subgoal premises prems2
+apply(insert prems2(1,2) prems1(3))
+apply(erule always_einv2req)
+apply simp
+  apply(rule always_disj_rule)
+  apply simp
+    apply(erule conjE)
+    subgoal premises prems3
+    apply(rule conjI)
+    apply(insert prems3(1,2))[1]
+      apply(rule weak_previous_LS5)
+      apply simp
+        apply(rule dual_since_L5)
+        apply simp
+          apply(erule conjE)
+          subgoal premises prems4
+          apply(rule conjI)
+          apply(insert prems4(1,2))[1]
+            apply(rule always_imp_refl)
+          apply(insert prems4(1,3))
+            apply(rule always_imp_refl)
+          done
+    apply(insert prems3(1,3))
+      apply(rule always_disj_rule)
+      apply simp
+        apply(erule conjE)
+        subgoal premises prems5
+        apply(rule conjI)
+        apply(insert prems5(1,2))[1]
+          apply(rule always_imp_refl)
+        apply(insert prems5(1,3))
+          apply assumption
+        done
+    done
+done
+done
+done
+
+lemma P6_1_inv_saving: "
+P6_1_inv_part t b_0 t1_0 b_1 A1 A2 A3 A4 s0 \<Longrightarrow>
+consecutive s0 s \<Longrightarrow>
+((((b_1 s0) \<or> ((\<not> (A3 s)) \<or> (A4 s))) \<and> ((b_1 s) --> (((t > 0) \<or> (\<not> (A1 s))) \<and> ((\<not> (A2 s)) \<or> ((b_0 s0) \<and> ((t1_0 s0) < t)))))) \<and> ((((t1_0 s) > 0) \<or> (\<not> (A1 s))) \<and> ((\<not> (A2 s)) \<or> ((b_0 s0) \<and> ((t1_0 s0) < (t1_0 s)))))) \<Longrightarrow>
+P6_1_inv_part t b_0 t1_0 b_1 A1 A2 A3 A4 s"unfolding P6_1_inv_part_def P6_1_part_def
+apply(simp add: P6_1_inv_saving_gen always_imp_refl)
+done
+
+lemma P6_1einv_imp_req: "
+P6_1_inv_part t b_0 t1_0 b_1 A1 A2 A3 A4 s \<Longrightarrow>
+toEnvP s \<Longrightarrow>
+True \<Longrightarrow>
+P6_1_part t A1 A2 A3 A4 s"unfolding P6_1_inv_part_def P6_1_part_def
+apply(simp add: P6_1einv_imp_req_gen always_imp_refl)
+done
+
+lemmas P6_1_used_patterns = P6_1_def always_def weak_previous_def dual_since_def 
+
+lemmas P6_1_inv_used_patterns = P6_1_inv_def always_inv_def weak_previous_def dual_since_def previous_inv_def dual_since_def dual_since_inv_def 
+
+lemmas P6_1_inv_part_used_patterns = P6_1_inv_part_def P6_1_inv_used_patterns
+
+lemmas P6_1_part_used_patterns = P6_1_part_def P6_1_used_patterns
+
+definition P6_2 where "P6_2 t A1 A2 A3 A4 A5 s \<equiv> (always (\<lambda> r2 r1 . ((weak_previous (\<lambda> r4 r3 . (dual_since t (\<lambda> r6 r5 . (\<not> (A2 r5))) (\<lambda> r6 r5 . (\<not> (A1 r5))) r4 r3)) r2 r1) \<or> ((\<not> (A3 r1)) \<or> (weak_until A4 A5 r2 r1)))) s)"
+
+definition P6_2_part where "P6_2_part t A1 A2 A3 A4 A5 s \<equiv> (P6_2 t A1 A2 A3 (\<lambda> s s1 . (A4 s1)) (\<lambda> s s1 . (A5 s1)) s)"
+
+definition P6_2_inv where "P6_2_inv t b_0 t1_0 b_1 w_0 A1 A2 A3 A4_1 A5_1 s \<equiv> (((always_inv (\<lambda> r2 r1 . ((weak_previous (\<lambda> r4 r3 . (dual_since t (\<lambda> r6 r5 . (\<not> (A2 r5))) (\<lambda> r6 r5 . (\<not> (A1 r5))) r4 r3)) r2 r1) \<or> ((\<not> (A3 r1)) \<or> (weak_until_inv w_0 A4_1 A5_1 r2 r1)))) s) \<and> (previous_inv b_1 (\<lambda> r4 r3 . (dual_since t (\<lambda> r6 r5 . (\<not> (A2 r5))) (\<lambda> r6 r5 . (\<not> (A1 r5))) r4 r3)) s)) \<and> (dual_since_inv t b_0 t1_0 (\<lambda> r6 r5 . (\<not> (A2 r5))) (\<lambda> r6 r5 . (\<not> (A1 r5))) s))"
+
+definition P6_2_inv_part where "P6_2_inv_part t b_0 t1_0 b_1 w_0 A1 A2 A3 A4 A5 s \<equiv> (P6_2_inv t b_0 t1_0 b_1 w_0 A1 A2 A3 (\<lambda> s s1 . (A4 s1)) (\<lambda> s s1 . (A5 s1)) s)"
+
+lemma P6_2_inv_saving_gen: "
+P6_2_inv t b_0 t1_0 b_1 w_0 A1 A2 A3 A4_1 A5_1 s0 \<Longrightarrow>
+consecutive s0 s \<Longrightarrow>
+(((((True \<and> True) \<and> (True \<and> ((always_imp s0 (A4_1 s0) (A4_1 s)) \<and> ((always_imp s0 (A5_1 s0) (A5_1 s)) \<and> ((\<not> (w_0 s0)) \<or> ((A5_1 s s) \<or> ((w_0 s) \<and> (A4_1 s s)))))))) \<and> (((b_1 s0) \<and> (True \<and> True)) \<or> ((\<not> (A3 s)) \<or> ((A5_1 s s) \<or> ((w_0 s) \<and> (A4_1 s s)))))) \<and> ((b_1 s) --> (((t > 0) \<or> (\<not> (A1 s))) \<and> ((\<not> (A2 s)) \<or> ((b_0 s0) \<and> (True \<and> (True \<and> ((t1_0 s0) < t)))))))) \<and> ((((t1_0 s) > 0) \<or> (\<not> (A1 s))) \<and> ((\<not> (A2 s)) \<or> ((b_0 s0) \<and> (True \<and> (True \<and> ((t1_0 s0) < (t1_0 s)))))))) \<Longrightarrow>
+P6_2_inv t b_0 t1_0 b_1 w_0 A1 A2 A3 A4_1 A5_1 s"
+unfolding P6_2_inv_def
+apply(erule conjE)
+apply(erule conjE)
+subgoal premises prems1
+apply(rule conjI)
+apply(insert prems1(1,2,4))[1]
+apply(erule conjE)
+apply(erule conjE)
+subgoal premises prems2
+apply(rule conjI)
+apply(insert prems2(1,2,4))[1]
+apply(erule always_rule)
+  apply simp
+  apply(erule conjE)
+  subgoal premises prems3
+  apply(rule conjI)
+  apply(insert prems3(1,2))[1]
+    apply(rule always_disj_rule)
+    apply simp
+      apply(erule conjE)
+      subgoal premises prems4
+      apply(rule conjI)
+      apply(insert prems4(1,2))[1]
+        apply(rule weak_previous_LS4)
+        apply simp
+          apply(rule dual_since_L4)
+          apply simp
+            apply(erule conjE)
+            subgoal premises prems5
+            apply(rule conjI)
+            apply(insert prems5(1,2))[1]
+              apply(rule always_imp_refl)
+            apply(insert prems5(1,3))
+              apply(rule always_imp_refl)
+            done
+      apply(insert prems4(1,3))
+        apply(rule always_disj_rule)
+        apply simp
+          apply(erule conjE)
+          subgoal premises prems6
+          apply(rule conjI)
+          apply(insert prems6(1,2))[1]
+            apply(rule always_imp_refl)
+          apply(insert prems6(1,3))
+            apply(rule weak_until_rule)
+            apply simp
+              apply(erule conjE)
+              subgoal premises prems7
+              apply(rule conjI)
+              apply(insert prems7(1,2))[1]
+                apply assumption
+              apply(insert prems7(1,3))
+                apply(erule conjE)
+                subgoal premises prems8
+                apply(rule conjI)
+                apply(insert prems8(1,2))[1]
+                  apply assumption
+                apply(insert prems8(1,3))
+                  apply(erule disjE)
+                  apply(rule disjI1)
+                    apply assumption
+                  apply(rule disjI2)
+                    apply(erule disjE)
+                    apply(rule disjI1)
+                      apply assumption
+                    apply(rule disjI2)
+                      apply(erule conjE)
+                      subgoal premises prems9
+                      apply(rule conjI)
+                      apply(insert prems9(1,2))[1]
+                        apply assumption
+                      apply(insert prems9(1,3))
+                        apply assumption
+                      done
+                done
+              done
+          done
+      done
+  apply(insert prems3(1,3))
+    apply(erule disjE)
+    apply(rule disjI1)
+      apply(rule weak_previous_one_point[OF prems2(3)])
+      apply simp
+        apply(erule conjE)
+        subgoal premises prems10
+        apply(rule conjI)
+        apply(insert prems10(1,2))[1]
+          apply assumption
+        apply(insert prems10(1,3))
+          apply(rule dual_since_L4)
+          apply simp
+            apply(erule conjE)
+            subgoal premises prems11
+            apply(rule conjI)
+            apply(insert prems11(1,2))[1]
+              apply(rule always_imp_refl)
+            apply(insert prems11(1,3))
+              apply(rule always_imp_refl)
+            done
+        done
+    apply(rule disjI2)
+      apply(erule disjE)
+      apply(rule disjI1)
+        apply assumption
+      apply(rule disjI2)
+        apply(rule weak_until_one_point)
+        apply simp
+          apply(erule disjE)
+          apply(rule disjI1)
+            apply assumption
+          apply(rule disjI2)
+            apply(erule conjE)
+            subgoal premises prems12
+            apply(rule conjI)
+            apply(insert prems12(1,2))[1]
+              apply assumption
+            apply(insert prems12(1,3))
+              apply assumption
+            done
+  done
+apply(insert prems2(1,3,5))
+  apply(erule previous_rule)
+  apply simp
+  apply(rule impI)
+  apply(erule impE)
+  apply assumption
+  subgoal premises prems13
+  apply(insert prems13(1,3))
+    apply(rule dual_since_L7[OF prems1(3)])
+    apply simp
+      apply(erule conjE)
+      subgoal premises prems14
+      apply(rule conjI)
+      apply(insert prems14(1,2))[1]
+        apply(erule disjE)
+        apply(rule disjI1)
+          apply assumption
+        apply(rule disjI2)
+          apply assumption
+      apply(insert prems14(1,3))
+        apply(erule disjE)
+        apply(rule disjI1)
+          apply assumption
+        apply(rule disjI2)
+          apply(erule conjE)
+          subgoal premises prems15
+          apply(rule conjI)
+          apply(insert prems15(1,2))[1]
+            apply assumption
+          apply(insert prems15(1,3))
+            apply(erule conjE)
+            subgoal premises prems16
+            apply(rule conjI)
+            apply(insert prems16(1,2))[1]
+              apply(rule always_imp_refl)
+            apply(insert prems16(1,3))
+              apply(erule conjE)
+              subgoal premises prems17
+              apply(rule conjI)
+              apply(insert prems17(1,2))[1]
+                apply(rule always_imp_refl)
+              apply(insert prems17(1,3))
+                apply assumption
+              done
+            done
+          done
+      done
+  done
+done
+apply(insert prems1(1,3,5))
+  apply(erule dual_since_one_point)
+  apply simp
+  apply(erule conjE)
+  subgoal premises prems18
+  apply(rule conjI)
+  apply(insert prems18(1,2))[1]
+    apply(erule disjE)
+    apply(rule disjI1)
+      apply assumption
+    apply(rule disjI2)
+      apply assumption
+  apply(insert prems18(1,3))
+    apply(erule disjE)
+    apply(rule disjI1)
+      apply assumption
+    apply(rule disjI2)
+      apply(erule conjE)
+      subgoal premises prems19
+      apply(rule conjI)
+      apply(insert prems19(1,2))[1]
+        apply assumption
+      apply(insert prems19(1,3))
+        apply(erule conjE)
+        subgoal premises prems20
+        apply(rule conjI)
+        apply(insert prems20(1,2))[1]
+          apply(rule always_imp_refl)
+        apply(insert prems20(1,3))
+          apply(erule conjE)
+          subgoal premises prems21
+          apply(rule conjI)
+          apply(insert prems21(1,2))[1]
+            apply(rule always_imp_refl)
+          apply(insert prems21(1,3))
+            apply assumption
+          done
+        done
+      done
+  done
+done
+done
+
+lemma P6_2einv_imp_req_gen: "
+P6_2_inv t b_0 t1_0 b_1 w_0 A1 A2 A3 A4_1 A5_1 s0 \<Longrightarrow>
+toEnvP s0 \<Longrightarrow>
+((True \<and> True) \<and> (True \<and> ((always_imp s0 (A4_1 s0) (A4 s0)) \<and> (always_imp s0 (A5_1 s0) (A5 s0))))) \<Longrightarrow>
+P6_2 t A1 A2 A3 A4 A5 s0"unfolding P6_2_inv_def P6_2_def
+subgoal premises prems1
+apply(insert prems1(1,2))
+apply(simp only: conj_assoc)
+apply(erule conjE)
+subgoal premises prems2
+apply(insert prems2(1,2) prems1(3))
+apply(erule always_einv2req)
+apply simp
+  apply(rule always_disj_rule)
+  apply simp
+    apply(erule conjE)
+    subgoal premises prems3
+    apply(rule conjI)
+    apply(insert prems3(1,2))[1]
+      apply(rule weak_previous_LS5)
+      apply simp
+        apply(rule dual_since_L5)
+        apply simp
+          apply(erule conjE)
+          subgoal premises prems4
+          apply(rule conjI)
+          apply(insert prems4(1,2))[1]
+            apply(rule always_imp_refl)
+          apply(insert prems4(1,3))
+            apply(rule always_imp_refl)
+          done
+    apply(insert prems3(1,3))
+      apply(rule always_disj_rule)
+      apply simp
+        apply(erule conjE)
+        subgoal premises prems5
+        apply(rule conjI)
+        apply(insert prems5(1,2))[1]
+          apply(rule always_imp_refl)
+        apply(insert prems5(1,3))
+          apply(rule weak_until_einv2req)
+          apply simp
+            apply(erule conjE)
+            subgoal premises prems6
+            apply(rule conjI)
+            apply(insert prems6(1,2))[1]
+              apply assumption
+            apply(insert prems6(1,3))
+              apply assumption
+            done
+        done
+    done
+done
+done
+done
+
+lemma P6_2_inv_saving: "
+P6_2_inv_part t b_0 t1_0 b_1 w_0 A1 A2 A3 A4 A5 s0 \<Longrightarrow>
+consecutive s0 s \<Longrightarrow>
+(((((\<not> (w_0 s0)) \<or> ((A5 s) \<or> ((w_0 s) \<and> (A4 s)))) \<and> ((b_1 s0) \<or> ((\<not> (A3 s)) \<or> ((A5 s) \<or> ((w_0 s) \<and> (A4 s)))))) \<and> ((b_1 s) --> (((t > 0) \<or> (\<not> (A1 s))) \<and> ((\<not> (A2 s)) \<or> ((b_0 s0) \<and> ((t1_0 s0) < t)))))) \<and> ((((t1_0 s) > 0) \<or> (\<not> (A1 s))) \<and> ((\<not> (A2 s)) \<or> ((b_0 s0) \<and> ((t1_0 s0) < (t1_0 s)))))) \<Longrightarrow>
+P6_2_inv_part t b_0 t1_0 b_1 w_0 A1 A2 A3 A4 A5 s"unfolding P6_2_inv_part_def P6_2_part_def
+apply(simp add: P6_2_inv_saving_gen always_imp_refl)
+done
+
+lemma P6_2einv_imp_req: "
+P6_2_inv_part t b_0 t1_0 b_1 w_0 A1 A2 A3 A4 A5 s \<Longrightarrow>
+toEnvP s \<Longrightarrow>
+True \<Longrightarrow>
+P6_2_part t A1 A2 A3 A4 A5 s"unfolding P6_2_inv_part_def P6_2_part_def
+apply(simp add: P6_2einv_imp_req_gen always_imp_refl)
+done
+
+lemmas P6_2_used_patterns = P6_2_def always_def weak_previous_def dual_since_def weak_until_def 
+
+lemmas P6_2_inv_used_patterns = P6_2_inv_def always_inv_def weak_previous_def dual_since_def weak_until_inv_def previous_inv_def dual_since_def dual_since_inv_def 
+
+lemmas P6_2_inv_part_used_patterns = P6_2_inv_part_def P6_2_inv_used_patterns
+
+lemmas P6_2_part_used_patterns = P6_2_part_def P6_2_used_patterns
 
 end
