examples/Turnstile/Requirements.thy
@@ -1,0 +1,56 @@
+theory Requirements
+  imports "../Derived_Patterns" Turnstile
+begin
+
+definition R1 where "R1 s \<equiv> toEnvP s \<and>
+P1_2_part 9 (\<lambda> s1. getVarBool s1 open' = True) (\<lambda> s2. getVarBool s2 PdOut') (\<lambda> s3. getVarBool s3 open' = True)
+ (\<lambda> s4. getVarBool s4 open' = False) s"
+
+definition Einv1 where "Einv1 s \<equiv> toEnvP s \<and>
+P1_2_inv_part 9 (\<lambda> s. getPstate s Controller' \<in> {Controller'isClosed', STOP}) 
+(\<lambda> s. if getPstate s Controller' = Controller'minimalOpened' \<and> getVarBool s passed' = True
+ then ltime s Controller' - 1 else 0)
+  (\<lambda> s1. getVarBool s1 open' = True) (\<lambda> s2. getVarBool s2 PdOut') (\<lambda> s3. getVarBool s3 open' = True)
+ (\<lambda> s4. getVarBool s4 open' = False) s"
+
+definition R2 where "R2 s \<equiv> toEnvP s \<and>
+always2_part (\<lambda> s1. getVarBool s1 open' = False) (\<lambda> s2. getVarBool s2 paid' = False)
+ (\<lambda> s2. getVarBool s2 open' = False) s"
+
+definition Einv2 where "Einv2 s \<equiv> toEnvP s \<and>
+always2_inv_part (\<lambda> s. getPstate s Controller' \<in> {Controller'minimalOpened', Controller'isOpened'})
+  (\<lambda> s1. getVarBool s1 open' = False) (\<lambda> s2. getVarBool s2 paid' = False)
+ (\<lambda> s2. getVarBool s2 open' = False) s"
+
+definition R3 where "R3 s \<equiv> toEnvP s \<and>
+always2_part (\<lambda> s1. getVarBool s1 open' = False \<and> getVarBool s1 paid' = False) (\<lambda> s2. getVarBool s2 paid' = True)
+(\<lambda> s2. getVarBool s2 open' = True) s"
+
+definition Einv3 where "Einv3 s \<equiv> toEnvP s \<and>
+always2_inv_part (\<lambda> s. getPstate s Controller' \<in> {Controller'minimalOpened', Controller'isOpened'})
+ (\<lambda> s1. getVarBool s1 open' = False \<and> getVarBool s1 paid' = False) (\<lambda> s2. getVarBool s2 paid' = True)
+(\<lambda> s2. getVarBool s2 open' = True) s"
+
+definition R4 where "R4 s \<equiv> toEnvP s \<and>
+P1_2_part 100 (\<lambda> s1. getVarBool s1 open' = False) (\<lambda> s2. getVarBool s2 open' = True)
+ (\<lambda> s3. getVarBool s3 open' = True) (\<lambda> s4. getVarBool s4 open' = False) s"
+
+definition Einv4 where "Einv4 s \<equiv> toEnvP s \<and>
+P1_2_inv_part 100  (\<lambda> s. getPstate s Controller' \<in> {Controller'minimalOpened', Controller'isOpened'})
+(\<lambda> s. if getPstate s Controller' = Controller'minimalOpened' then ltime s Controller'
+ else if getPstate s Controller' = Controller'isOpened' then ltime s Controller' + 90 else 0)
+ (\<lambda> s1. getVarBool s1 open' = False) (\<lambda> s2. getVarBool s2 open' = True)
+ (\<lambda> s3. getVarBool s3 open' = True) (\<lambda> s4. getVarBool s4 open' = False) s"
+
+definition R5 where "R5 s \<equiv> toEnvP s \<and>
+P2_2_part 10 (\<lambda> s1. getVarBool s1 open' = False) (\<lambda> s2. getVarBool s2 open' = True)
+ (\<lambda> s3. getVarBool s3 open' = True)  s"
+
+definition R6 where "R6 s \<equiv> toEnvP s \<and>
+always_part (\<lambda> s1. getVarBool s1 opened' \<longrightarrow> getVarBool s1 enter') s"
+
+definition R7 where "R7 s \<equiv> toEnvP s \<and>
+always2_part (\<lambda> s1. getVarBool s1 enter' = True) (\<lambda> s2. getVarBool s2 enter' = False)
+ (\<lambda> s2. getVarBool s2 reset' = True) s"
+
+end
